coq-osiris/examples/proofs/splay.v
@@ -109,25 +109,9 @@ Definition zlt {A} (z1 z2 : zipper A) :=
   {| wf_relation := zlt |}.
 Next Obligation. constructor; unfold zlt; apply wf_inverse_image, lt_wf. Qed.
 
-(* Datatype instance for [tree] *)
-
-(* LATER: Can this be generated during translation? *)
-
-Definition Leaf_ {A} : sigT (data_constructor (tree A)) :=
-  existT [] Leaf.
-
-Definition Node_ {A} : sigT (data_constructor (tree A)) :=
-  existT [tree A; A; tree A] Node.
-
-#[global] Instance tree_datatype `{Encode A} : DataType (tree A) :=
-  { data_signature :=
-      <["Leaf" := Leaf_ (A := A) ]>
-        (<["Node" := Node_ (A := A) ]> ∅) }.
-
 (* -------------------------------------------------------------------------- *)
 
-(* Encodings *)
-
+Section encode.
 Local Fixpoint encode_tree `{Encode A} (t : tree A) : val :=
   match t with
   | Leaf =>
@@ -140,17 +124,70 @@ Local Fixpoint encode_tree `{Encode A} (t : tree A) : val :=
   { encode := encode_tree }.
 
 Local Fixpoint encode_zipper `{Encode A} (z : zipper A) : val :=
+  let (c, l) :=
+    (match z with
+    | Root =>
+        ("Root", nil)
+    | NodeL z1 x t2 =>
+        ("NodeL", [encode_zipper z1; #x; #t2])
+    | NodeR t1 x z2 =>
+        ("NodeR", [ #t1; #x; encode_zipper z2])
+    end)
+  in
+  VData c l.
+
+Definition zipper_tag `{Encode A} (z : zipper A) : string :=
   match z with
   | Root =>
-      VConstant "Root"
+      "Root"
   | NodeL z1 x t2 =>
-      VData "NodeL" [encode_zipper z1; #x; #t2]
+      "NodeL"
   | NodeR t1 x z2 =>
-      VData "NodeR" [ #t1; #x; encode_zipper z2]
+      "NodeR"
   end.
+
+Definition zipper_data `{Encode A} (z : zipper A) : list val :=
+  match z with
+  | Root =>
+      nil
+  | NodeL z1 x t2 =>
+      [encode_zipper z1; #x; #t2]
+  | NodeR t1 x z2 =>
+      [ #t1; #x; encode_zipper z2]
+  end.
+
+Lemma unfold_encode_zipper `{Encode A} (z : zipper A) :
+  encode_zipper z = VData (zipper_tag z) (zipper_data z).
+Proof.
+  induction z; eauto.
+Qed.
+
+Definition tree_tag `{Encode A} (z : tree A) : string :=
+  match z with
+  | Node _ _ _ =>
+      "Node"
+  | Leaf =>
+      "Leaf"
+  end.
+
+Definition tree_data `{Encode A} (z : tree A) : list val :=
+  match z with
+  | Leaf => nil
+  | Node z1 x t2 => [ #z1; #x; #t2]
+  end.
+
+Lemma unfold_encode_tree `{Encode A} (t : tree A) :
+  encode_tree t = VData (tree_tag t) (tree_data t).
+Proof.
+  induction t; eauto.
+Qed.
+
+Opaque encode_zipper.
+Opaque encode_tree.
 
 #[global] Instance Encode_zipper `{Encode A} : Encode (zipper A) :=
   { encode := encode_zipper }.
+End encode.
 
 (* -------------------------------------------------------------------------- *)
 
@@ -174,7 +211,44 @@ Section BST.
   Definition bst (t : tree A) :=
     Sorted lt (fringe t).
 
+  Notation "xs '≺' ys" := (pairwise lt xs ys) (at level 80).
+
+  (* The following lemmas provide an alternative characterization of binary
+    search trees. If the predicate [bst t] was inductively defined, then
+    these two statements would correspond the two constructors (and their
+    inversion principle). *)
+
+  Lemma bst_Leaf_iff :
+    bst Leaf ↔ True.
+  Proof.
+    unfold bst. simpl fringe. rewrite Sorted_empty_iff. auto.
+  Qed.
+
+  Lemma cons_is_app x (l1 : list A) : x :: l1 = [x] ++ l1. Proof. auto. Qed.
+
+  Lemma bst_Node_iff l x r :
+    bst (Node l x r) ↔
+    bst l ∧ bst r ∧ fringe l ≺ [x] ∧ [x] ≺ fringe r.
+  Proof.
+    unfold bst. simpl fringe.
+    repeat (first [ rewrite Sorted_app_iff
+                  | rewrite Sorted_singleton_iff
+                  | rewrite cons_is_app; rewrite Sorted_app_iff
+                  | rewrite pairwise_app_right_iff]).
+    pose proof (@pairwise_transitive_singleton _ lt _ (fringe l) x (fringe r)).
+    tauto.
+  Qed.
+
 End BST.
+
+Ltac destruct_bst_Node :=
+  lazymatch goal with h: bst _ (Node _ _ _) |- _ =>
+    rewrite bst_Node_iff in h; try typeclasses eauto;
+    destruct h as (?&?&?&?)
+  end.
+
+(* -------------------------------------------------------------------------- *)
+
 
 (* -------------------------------------------------------------------------- *)
 
@@ -234,13 +308,206 @@ Local Ltac prove_same_fringe :=
           rewrite <- ?app_assoc) ;
   eauto.
 
-(* -------------------------------------------------------------------------- *)
-
 Section splay_proofs.
 
 (* Top-level environment of [splay]. *)
 
+Arguments encode.encode : simpl never.
+
 (* -------------------------------------------------------------------------- *)
+
+Ltac pats :=
+  repeat first [
+      eapply pats_PNil; [ eauto ]
+    | eapply pats_PCons; [ eauto | simpl; intros ]
+    ].
+
+Definition pLeaf := PConstant "Leaf".
+
+Lemma pat_pLeaf `{Encode A} η v (t : tree A) (φ : env -> Prop) :
+  v = #t →
+  (t = Leaf -> φ η) ->
+  pattern η pLeaf v φ (t <> Leaf).
+Proof.
+  intros; subst.
+  destruct t.
+  { eapply pattern_exn_mono.
+    { eapply pat_PData_eq; pats. }
+    destruct 1. }
+  { eapply pattern_exn_mono.
+    { eapply pat_PData_neq; auto. }
+    congruence. }
+Qed.
+
+Ltac pat_pLeaf :=
+  eapply pat_pLeaf; first solve [encode].
+
+Definition pNode (p1 p2 p3 : syntax.pat) :=
+  PData "Node" [p1; p2; p3].
+
+Lemma pat_pNode `{Encode A} (η : env) (v : val) (t : tree A)
+  (p1 p2 p3 : syntax.pat) (φ : env -> Prop)
+  (ψ1 : tree A -> Prop) (ψ2 : A -> Prop) (ψ3 : tree A -> Prop)
+  :
+  v = #t ->
+  (∀ (t1 : tree A) (a : A) (t2 : tree A),
+      t = Node t1 a t2 →
+      pattern η p1 #t1
+        (λ η', pattern η' p2 #a
+            (λ η', pattern η' p3 #t2 φ (ψ3 t2))
+            (ψ2 a))
+        (ψ1 t1)) ->
+  pattern η (pNode p1 p2 p3) v φ
+    (t = Leaf \/ (exists t1 a t2, t = Node t1 a t2 /\ (ψ1 t1 \/ ψ2 a \/ ψ3 t2))).
+Proof.
+  intros -> Hcov.
+  destruct t; eapply pattern_exn_mono.
+  { eapply pat_PData_neq; eauto. }
+  { auto. }
+  { eapply pat_PData_eq; pats ; eauto. }
+  { clear; right; do 3 eexists; split; [ reflexivity | tauto ]. }
+Qed.
+
+Ltac pat_pNode :=
+  eapply pat_pNode; first solve [encode].
+
+Definition pRoot := PConstant "Root".
+
+Lemma pat_pRoot `{Encode A} η v (z : zipper A) (φ : env -> Prop) :
+  v = #z →
+  (z = Root -> φ η) ->
+  pattern η pRoot v φ (z <> Root).
+Proof.
+  intros; subst.
+  destruct z.
+  { eapply pattern_exn_mono.
+    { eapply pat_PData_eq; pats. }
+    destruct 1. }
+  { eapply pattern_exn_mono.
+    { eapply pat_PData_neq; auto. }
+    congruence. }
+  { eapply pattern_exn_mono.
+    { eapply pat_PData_neq; auto. }
+    congruence. }
+Qed.
+
+Ltac pat_pRoot :=
+  eapply pat_pRoot; first solve [encode].
+
+Definition pNodeL (p1 p2 p3 : syntax.pat) :=
+  PData "NodeL" [p1; p2; p3].
+
+Lemma pat_pNodeL `{Encode A} (η : env) (v : val) (z : zipper A)
+  (p1 p2 p3 : syntax.pat) (φ : env -> Prop)
+  (ψ1 : zipper A -> Prop) (ψ2 : A -> Prop) (ψ3 : tree A -> Prop)
+  :
+  v = #z ->
+  (∀ (z' : zipper A) (a : A) (t : tree A),
+      z = NodeL z' a t →
+      pattern η p1 #z' (λ η', pattern η' p2 #a (λ η', pattern η' p3 #t φ (ψ3 t)) (ψ2 a)) (ψ1 z')) ->
+  pattern η (pNodeL p1 p2 p3) v φ (z = Root \/
+                                 (exists a1 a2 a3, z = NodeR a1 a2 a3) \/
+                                 (exists z' a t, z = NodeL z' a t /\ (ψ1 z' \/ ψ2 a \/ ψ3 t))).
+Proof.
+  intros -> Hcov.
+  destruct z; eapply pattern_exn_mono.
+  { eapply pat_PData_neq; eauto. }
+  { auto. }
+  { eapply pat_PData_eq; pats; eauto. }
+  { clear; do 2 right; do 3 eexists; split; [ reflexivity | tauto ]. }
+  { eapply pat_PData_neq; eauto. }
+  { right; left; eauto. }
+Qed.
+
+Ltac pat_pNodeL :=
+  eapply pat_pNodeL; first solve [encode].
+
+Definition pNodeR (p1 p2 p3 : syntax.pat) :=
+  PData "NodeR" [p1; p2; p3].
+
+Lemma pat_pNodeR `{Encode A} (η : env) (v : val) (z : zipper A)
+  (p1 p2 p3 : syntax.pat) (φ : env -> Prop)
+  (ψ1 : tree A -> Prop) (ψ2 : A -> Prop) (ψ3 : zipper A -> Prop)
+  :
+  v = #z ->
+  (∀ (t : tree A) (a : A) (z' : zipper A),
+      z = NodeR t a z' →
+      pattern η p1 #t (λ η', pattern η' p2 #a (λ η', pattern η' p3 #z' φ (ψ3 z')) (ψ2 a)) (ψ1 t)) ->
+  pattern η (pNodeR p1 p2 p3) v φ (z = Root \/
+                                 (exists a1 a2 a3, z = NodeL a1 a2 a3) \/
+                                 (exists t a z', z = NodeR t a z' /\ (ψ1 t \/ ψ2 a \/ ψ3 z'))).
+Proof.
+  intros -> Hcov.
+  destruct z; eapply pattern_exn_mono.
+  { eapply pat_PData_neq; eauto. }
+  { auto. }
+  { eapply pat_PData_neq; eauto. }
+  { right; left; eauto. }
+  { eapply pat_PData_eq; pats. }
+  { clear; right; right; do 3 eexists; split; [ reflexivity | tauto ]. }
+Qed.
+
+Ltac pat_pNodeR :=
+  eapply pat_pNodeR; first solve [encode].
+
+Ltac pattern_hook ::=
+  first
+    [ pat_pRoot
+    | pat_pNodeL
+    | pat_pNodeR
+    | pat_pLeaf
+    | pat_pNode
+    ].
+
+Lemma solve_encode_Leaf `{Encode A} (t : tree A) :
+  Leaf = t →
+  VConstant "Leaf" = #t.
+Proof.
+  intros. subst. eauto.
+Qed.
+
+Lemma solve_encode_Node `{Encode A} t1 x t2 (t : tree A) vt1 vx vt2 :
+  Node t1 x t2 = t →
+  vt1 = #t1 →
+  vx = #x →
+  vt2 = #t2 →
+  VData "Node" [vt1; vx; vt2] = #t.
+Proof.
+  intros. subst. eauto.
+Qed.
+
+Local Hint Resolve solve_encode_Leaf solve_encode_Node : encode.
+
+Lemma solve_encode_Root `{Encode A} (z : zipper A) :
+  Root = z →
+  VConstant "Root" = #z.
+Proof.
+  intros. subst. eauto.
+Qed.
+
+Lemma solve_encode_NodeL `{Encode A} z1 x t2 (z : zipper A) vz1 vx vt2 :
+  NodeL z1 x t2 = z →
+  vz1 = #z1 →
+  vx = #x →
+  vt2 = #t2 →
+  VData "NodeL" [vz1; vx; vt2] = #z.
+Proof.
+  intros. subst. eauto.
+Qed.
+
+Lemma solve_encode_NodeR `{Encode A} t1 x z2 (z : zipper A) vt1 vx vz2 :
+  NodeR t1 x z2 = z →
+  vt1 = #t1 →
+  vx = #x →
+  vz2 = #z2 →
+  VData "NodeR" [vt1; vx; vz2] = #z.
+Proof.
+  intros. subst. eauto.
+Qed.
+
+Local Hint Resolve
+  solve_encode_Root solve_encode_NodeL solve_encode_NodeR
+  : encode.
 
 Lemma Splay_spec :
   splay_spec
@@ -255,24 +522,63 @@ Proof.
          (l, x, r, ctx)).
 
   (* Recursion, with decreasing depth of zipper. *)
-  recursion { measure snd } ∀ (l, x, r, ctx).
-
+  recursion { measure snd } ∀ (l, x, r, ctx). (* FIXME: VCloRec exposure. *)
   clear l x r ctx; intros splay [[[l x] r] ctx] IH.
 
   (* Match to destruct the argument tuple *)
-  eval_match; pure_match.
+  eapply pure_eval_match. { pure_path. }
 
   (* Match on [ctx] *)
-  eval_match.
+  pure_match.
+  eapply pure_eval_match. { pure_path. }
 
-  destruct ctx eqn: Hctx.
-  { (* Case: [ctx] matches [Root] *)
-    pure_match. pure_data. prove_same_fringe. }
+  pure_match. (* Very slow. TODO Profile and fix. *)
 
-  (* TODO: Generate custom match cases like before *)
+  (* Case: [ctx] matches [Root] *)
+  { pure_data. }
 
-  (* We should be able to continually apply [pure_match_cons]. *)
-Admitted.
+  (* Case: [ctx] matches [NodeL (Root, y, ry)] *)
+  { pure_data.
+    prove_same_fringe. }
+
+  (* Case: [ctx] matches [NodeL (NodeL (up, z, rz), y, ry)] *)
+  { eapply pure_eval_app. pure_path.
+    eapply pure_eval_quadruple.
+    pure_path. pure_path. pure_data. pure_path.
+    eapply pure_mono.
+    { eapply IH; cbn; unfold zlt; subst; auto with arith. }
+    simpl; intros ? ->.
+    prove_same_fringe. }
+
+  (* Case: [ctx] matches [NodeL (NodeR (lz, z, up), y, ry)] *)
+  { eapply pure_eval_app. pure_path.
+    eapply pure_eval_quadruple. pure_data. pure_path. pure_data. pure_path.
+    eapply pure_mono.
+    { eapply IH; cbn; unfold zlt; subst; auto with arith. }
+    simpl; intros ? ->.
+    prove_same_fringe. }
+
+  (* Case: [ctx] matches [NodeR (ly, y, Root)] *)
+  { pure_data.
+    prove_same_fringe. }
+
+  (* Case: [ctx] matches [NodeR (ly, y, NodeL (up, z, rz))] *)
+  { eapply pure_eval_app.
+    pure_path.
+    eapply pure_eval_quadruple. pure_data. pure_path. pure_data. pure_path.
+    eapply pure_mono.
+    { eapply IH; cbn; unfold zlt; subst; auto with arith. }
+    intros ? ->.
+    prove_same_fringe. }
+
+  (* Case: [ctx] matches [NodeR (ly, y, NodeR (lz, z, up))] *)
+  { eapply pure_eval_app. pure_path.
+    eapply pure_eval_quadruple. pure_data. pure_path. pure_path. pure_path.
+    eapply pure_mono.
+    { eapply IH; cbn; unfold zlt; subst; auto with arith. }
+    intros ? ->.
+    prove_same_fringe. }
+Qed.
 
 Lemma Splay_leaf_spec splay :
   splay_spec splay ->
@@ -280,7 +586,35 @@ Lemma Splay_leaf_spec splay :
     (VClo ("splay" ~> splay; stdlib_env) __fun4).
 Proof.
   unfold splay_leaf_spec.
-Admitted.
+  intros Hsplay A H ctx.
+  pure_enter.
+  (* Match on [ctx] *)
+  eapply pure_eval_match. { pure_path; reflexivity. }
+  pure_match.
+
+  (* Case: [ctx] matches [Root] *)
+  { pure_const. reflexivity. }
+
+  (* Case: [ctx] matches [NodeL (up, x, r)] *)
+  { eapply pure_eval_app. pure_path. (* What does [pure_path] do? *)
+    Unshelve.
+    eapply pure_eval_quadruple.
+    eapply pure_eval_const.
+    apply (@solve_encode_Leaf A); reflexivity. (* Todo: weird *)
+
+    pure_path. pure_path. pure_path.
+    unfold splay_spec in Hsplay.
+    specialize (Hsplay _ _ z' Leaf a t).
+    apply Hsplay. }
+
+  (* Case: [ctx] matches [NodeR (l, x, up)] *)
+  { eapply pure_eval_app. pure_path. eapply pure_eval_quadruple.
+    pure_path. pure_path. eapply pure_eval_const.
+    apply (@solve_encode_Leaf A). reflexivity.
+    pure_path.
+    specialize (Hsplay _ _ z' t a Leaf).
+    apply Hsplay. }
+Qed.
 
 Lemma Zlookup_spec splay splay_leaf :
   splay_leaf_spec splay_leaf ->
@@ -302,10 +636,11 @@ Proof.
        member le x (fringe t) oy ∧ fringe t' = fringe (fill ctx t))
        (t, x, ctx)).
 
-  recursion { measure (fun x => fst (fst x)) } ∀ (t, x, ctx).
+  recursion { measure (fun x => fst (fst x)) } ∀ (t, x, ctx) gen (fun x => bst (strict le) x.1.1);
+   first done.
 
-  clear Hbst t x ctx; intros zlookup [[t x] ctx] IH.
-  simpl in *. fold eval.
+  clear x ctx; intros zlookup [(t' & x) ctx] IH.
+  simpl in *. fold eval. clear Hbst; intros Hbst.
 
   (* Match on tuple argument *)
   eapply pure_eval_match. { pure_path. }
@@ -313,6 +648,85 @@ Proof.
   (* Match on [t] *)
   eapply pure_eval_match. { pure_path. }
   pure_match.
+
+  (* Case: [t] matches [Leaf] *)
+  { eapply pure_eval_pair. pure_const.
+    eapply pure_eval_app. pure_path. pure_path.
+    change (encode_zipper ctx) with (# ctx); done.
+    simple eapply pure_mono; first eapply Hsplay_leaf.
+    split; [ intros | auto]. repeat intro; by eapply not_elem_of_nil. }
+
+  (* Case: [t] matches [Node (l, y, r)] *)
+  { destruct_bst_Node.
+
+    eapply pure_eval_let.
+    { (* Evaluate rhs of [let c = ..] *)
+      eapply pure_eval_app2.
+      { pure_path; reflexivity. }
+      { pure_path; reflexivity. }
+      { pure_path; reflexivity. }
+      unfold pure_call2.
+      unfold compare_spec in Hcompare.
+      eapply Hcompare. }
+    (* Evaluate continuation expression after let *)
+    intros c (? & Hlt & Heq & Hgt).
+    eapply pure_eval_ifthenelse.
+    { (* Evalute comparison operation *)
+      eapply pure_eval_EOpLt.
+      { pure_path. }
+      { eapply total_eval_int. reflexivity. }
+      { assumption. }
+      { representable. } }
+
+    { (* Case: [c < 0] *)
+      intro Clt0.
+      eapply pure_eval_app. pure_path.
+      eapply pure_eval_triple. pure_path. pure_path. pure_data.
+      eapply pure_mono.
+      { eapply IH with (y := (t1, x, NodeL ctx a t2));
+          unfold tlt, tree_depth; auto with arith. }
+      intros [oy t'] [??]; simpl in *.
+      split; [ | assumption ].
+      - apply bst_member_left; representable. }
+
+    { (* Case: [c >= 0] *)
+      intros Cge0.
+      eapply pure_eval_ifthenelse.
+      { (* Evaluate second comparison operation *)
+        eapply pure_eval_EOpGt.
+        { pure_path. }
+        (* TODO *)
+        { eapply pure_eval_int. reflexivity. }
+        { assumption. }
+        { representable. } }
+
+      { (* Subcase: [c > 0] *)
+        intros Cgt0.
+        eapply pure_eval_app. pure_path.
+        eapply pure_eval_triple. pure_path. pure_path. pure_data.
+        pure_call.
+        { eapply IH with (y := (t2, x, NodeR t1 a ctx)).
+          { unfold tlt, tree_depth; lia. }
+          { auto. } }
+        intros [oy t'] [??]; simpl in *.
+        split.
+        - apply bst_member_right; representable.
+          apply Hgt; apply Z.gt_lt; auto.
+        - assumption. }
+
+      { (* Subcase: [c <= 0] *)
+        intros Cle0.
+        (* Deduce [c = 0] *)
+        eapply pure_eval_pair. pure_data.
+        eapply pure_eval_app. pure_path.
+        eapply pure_eval_quadruple. pure_path. pure_path. pure_path. pure_path.
+        pure_call.
+        intros. split; [ split | ].
+        - apply Heq. lia.
+        - apply elem_of_app; right; apply elem_of_cons; left; reflexivity.
+        - assumption. } } }
+Qed.
+
 
   (* Case: [t] matches [Leaf] *)
 Admitted.
