coq-osiris/theories/program_logic/pure/eval_rules.v
@@ -1,31 +1,13 @@
 From osiris Require Import base.
 From osiris.lang Require Import locations lang.
-From osiris.semantics Require Import code eval simplification.
+From osiris.semantics Require Import semantics.
+From osiris.program_logic.pure Require Import simp_tactics
+  wp notation total_rules pattern_rules.
 
-From osiris.program_logic.pure Require Import wp notation total_rules.
-
+(* FIXME : Why is the import weird here? *)
+Tactic Notation "simp" := (simp).
 
 Section ceval_rules.
-
-  (** [CEval] evaluation *)
-
-  Context {A} {EncA: Encode A}.
-
-  Lemma pure_CEval {E η e k} (φ : A → Prop) (ψ : E → Prop) :
-    pure (try2 (eval η e) k) φ ψ →
-    pure (Stop CEval (η, e) k) φ ψ.
-  Proof.
-    intros. eapply pure_wp_det_may_backward; eauto. repeat constructor.
-    by intros m' ->%pure.invert_may_eval.
-  Qed.
-
-  Lemma pure_CEval_inject2 {η e φ ψ} :
-    pure (A := A) (eval η e) φ ψ →
-    pure (Stop CEval (η, e) inject2) φ ψ.
-  Proof.
-    intros He. eapply pure_CEval, pure_try2; try done;
-    eauto using pure_ret, pure_throw.
-  Qed.
 
 End ceval_rules.
 
@@ -36,25 +18,12 @@ End ceval_rules.
 (* Fun with data constructors: we can know the destructor as long as we
    have the signature of the algebraic datatype. *)
 
-(* The type of a data constructor can be built from the list of
-   constructor argument types. *)
-Fixpoint data_constructor A (x : list Type) : Type :=
-  match x with
-    | nil => A
-    | hd :: tl => hd -> data_constructor A tl
-  end.
-
-(* A signature for a constructor that builds type [A]. *)
-Definition signature {A} : Type := sigT (data_constructor A).
-
-(* Data types is a map from string (constructor name) to the type signatures
-  of the constructors. *)
-Class DataType (A : Type) :=
-  { data_signature : gmap.gmap string (@signature A); }.
+(* An encodable type. *)
+Definition encodable : Type := sigT Encode.
+Notation π1 := (projT1).
+Notation π2 := (projT2).
 
 (* -------------------------------------------------------------------------- *)
-
-(* TODO: Move *)
 
 (* Utility *)
 
@@ -65,18 +34,19 @@ From Equations Require Import Equations.
 Section hlist.
   Set Implicit Arguments.
 
+  (* FIXME : [A] -> [U];
+             [B] -> [el] *)
   Inductive hlist (A : Type) (B : A -> Type) : list A -> Type :=
   | HNil : hlist B nil
   | HCons : forall (x : A) (ls : list A), B x -> hlist B ls -> hlist B (x :: ls).
+
   Arguments HNil {A B}.
   Arguments HCons {A B x ls}.
 
-  (* Append for heterogeneous lists. *)
-
-  Equations happ (A B : list Type) :
-    hlist (fun T : Type => T) A ->
-    hlist (fun T : Type => T) B ->
-    hlist (fun T : Type => T) (A ++ B) :=
+  Equations happ (A B : list encodable) :
+    hlist π1 A ->
+    hlist π1 B ->
+    hlist π1 (A ++ B) :=
   happ HNil m := m;
   happ (HCons a l1) m := HCons a (happ l1 m).
 
@@ -89,59 +59,20 @@ Arguments HCons {A B x ls}.
 
 (* Construct a data type [A] given its signature, data constructor and arguments. *)
 
-Equations build_constructor {A}
-  (Σ : list Type)
-  (constr : data_constructor A Σ)
-  (data : hlist (fun T : Type => T) Σ)
-  : A :=
+Equations build_constructor
+  (Σ : list (sigT Encode))
+  (* (constr : data_constructor s Σ) *)
+  (data : hlist π1 Σ) : list val :=
   (* When there are no arguments left, the construction is immediate. *)
-  @build_constructor _ nil constr HNil := constr;
+  @build_constructor nil HNil := [];
 
   (* Peel off an argument of the signature and apply to the constructor. *)
-  @build_constructor _ (τ :: tl) constr (HCons v vtl) :=
-    (build_constructor (Σ := tl) (constr v) vtl).
+  @build_constructor (τ :: tl) (HCons v vtl) :=
+    encode (Encode := π2 τ) v ::
+      (build_constructor (Σ := tl) vtl).
 
-(* TODO Comment *)
-
-Fixpoint eval_data_aux {A X}
-  (* FIXME: Change argument names *)
-  (v : list expr)
-  (η : env)
-  (φ : A -> Prop) (ψ : exn -> Prop)
-  (t : list Type)
-  (constr : data_constructor A X)
-  (acc_t : list Type)
-  (acc : hlist (fun T : Type => T) acc_t)
-  : Prop :=
-  match v, t with
-  | hd :: tl, hd_t :: tl_t =>
-      ∃ (EncX : Encode hd_t) x,
-      pure
-        (eval η hd)
-        (fun y : hd_t =>
-          y = x /\
-          @eval_data_aux _ _ tl η φ ψ
-            tl_t
-            constr
-            (acc_t ++ [hd_t])
-            (happ acc (HCons x HNil))) ⊥
-  | nil, nil =>
-      exists (eq_X : acc_t = X),
-      φ (@build_constructor _ acc_t
-           (eq_rect_r
-              (fun X => data_constructor A X)
-              constr eq_X) acc)
-  | _ , _ => False
-end.
-
-Arguments eval_data_aux {A X} _ _ _ _ _ _ _ _.
-
-(* Evaluate a list of expressions into a data type according to the signature. *)
-
-Definition eval_data {A}
-  (e : list expr) (η : env) (φ : A -> Prop) (ψ : exn -> Prop) (Σ : @eval_rules.signature A)
-  := @eval_data_aux A _ e η φ ψ (projT1 Σ) (projT2 Σ) nil HNil.
-
+(* -------------------------------------------------------------------------- *)
+(** * Evaluation of Datatypes *)
 (* -------------------------------------------------------------------------- *)
 
 Lemma pure_eval_data_eq `{Encode A} a η c e (ψ : A -> Prop) ζ:
@@ -158,65 +89,88 @@ Proof.
   intros l <-; apply pure_wp_ret. eauto with pure.
 Qed.
 
-Require Import Coq.Logic.EqdepFacts.
-
-Lemma pure_eval_data {A} `{Encode A, DataType A} η
-  c hd tl (φ : _ -> Prop) ψ
-  (signature : sigT (data_constructor A)) :
-  data_signature !! c = Some signature ->
-  eval_data (hd :: tl) η φ ψ signature ->
-  pure (A := A) (eval η (EData c (hd :: tl))) φ ψ.
+Lemma pure_eval_data_eq2 Σ a η c e (ψ : val -> Prop) ζ:
+  pure_wp
+    (evals η e)
+    (λ x, VData c (@build_constructor Σ a) = VData c x) ζ ->
+  ψ (VData c (@build_constructor Σ a)) ->
+  pure (eval η (EData c e)) ψ ζ.
 Proof.
-  intros Hsig Heval.
+  intros Hwp Hψ.
   simpl_eval.
-  unfold eval_data in Heval.
-  simp eval_data_aux in Heval.
-  destruct signature as (t & constr); clear Hsig.
+  eapply pure_wp_bind.
+  eapply pure_wp_mono; eauto.
+  intros l <-; apply pure_wp_ret. eauto with pure.
+Qed.
 
-  (* Case analysis on the list type *)
-  destruct t.
-  { simpl in Heval. done. }
-
-  revert constr Heval.
-  induction t.
-
-  { (* Base case *)
-    intros constr Heval.
-    destruct Heval as (?&?&?).
-    eapply pure_wp_Par_val_left, pure_wp_mono; eauto.
-    intros a' Hret; red in Hret; destruct Hret as (?&?&?&?).
-    simpl in H4; subst.
-    destruct tl; simp eval_data_aux in H4; cycle 1.
-    { unfold eval_data_aux in H4; done. }
-
-    cbn; simpl_evals; do 2 apply pure_wp_ret.
-    cbn in *; destruct H4 as (?&?).
-    simp happ in H2.
-
-    simp build_constructor in H2.
-    red; eexists _; split; eauto; unfold eq_rect_r.
-    rewrite <- Eqdep.EqdepTheory.eq_rect_eq.
-
-    (* TODO: Customize the instance for [Encode A]. *)
-    (* VData c [#x0] = #(constr x0) *)
-    admit. }
-
-  (* Inductive case *)
-
-  intros constr Heval.
-  destruct Heval as (?&?&?).
-  eapply pure_wp_Par_val_left, pure_wp_mono; eauto.
-  intros a' Hret; red in Hret; destruct Hret as (?&?&?&?).
-  simpl in H4. subst. destruct tl; simp eval_data_aux in H4.
-  { by unfold eval_data_aux in H4. }
-
-  cbn. simpl_evals.
-  eapply pure_wp_mono.
-
-Admitted.
+(* -------------------------------------------------------------------------- *)
 
 (* -------------------------------------------------------------------------- *)
 (** *Evaluating function calls *)
+(* -------------------------------------------------------------------------- *)
+
+(* This trivial lemma gives the user a chance to prove that the actual
+   argument [v'2] is in fact the encoding of some value [x]. The subgoal
+   [v'2 = #x] is typically solved by the tactic [encode]. Solving this
+   subgoal instantiates both the metavariable [x] and the metavariable [X],
+   which is the type of [x]. *)
+
+Lemma pure_call `{Encode X} `{Encode Y}
+  (φ : Y → Prop) v1 v'2 (x : X) :
+  v'2 = #x →
+  pure (call v1 #x) φ ⊥ →
+  pure (call v1 v'2) φ ⊥.
+Proof.
+  intros. subst. eauto.
+Qed.
+
+(* This lemma combines [pure_enc_consequence] and [pure_call]. *)
+
+Lemma pure_call_consequence `{Encode X} `{Encode Y}
+  (φ ψ : Y → Prop) v1 v'2 (x : X) :
+  v'2 = #x →
+  pure (call v1 #x) φ ⊥ →
+  (∀ y, φ y → ψ y) →
+  pure (call v1 v'2) ψ ⊥.
+Proof.
+  eauto using pure_mono, pure_call.
+Qed.
+
+(* The following two lemmas paraphrase the definition of [call] in eval.v.
+   When applied to a goal of the form [simp (call v1 v2) _] where [v1] is
+   a concrete closure (as opposed to a rigid metavariable), they step into
+   the call. *)
+
+Lemma pure_enter_call_VClo `{Encode Y} η a v2 (φ : Y → Prop) ψ :
+  pure (acall η a v2) φ ψ ->
+  pure (call (VClo η a) v2) φ ψ.
+Proof.
+  tauto.
+Qed.
+
+Lemma pure_enter_call_VCloRec `{Encode Y} η rbs g x e v2 (φ : Y → Prop) ψ :
+  lookup_rec_bindings rbs g = ret (AnonFun x e) ->
+  pure (eval ((x, v2) :: eval_rec_bindings η rbs ++ η) e) φ ψ ->
+  pure (call (VCloRec η rbs g) v2) φ ψ.
+Proof.
+  intros Hlookup Hpure.
+  simpl; rewrite Hlookup.
+  eapply pure_CEval; rewrite try2_ret_right.
+  done.
+Qed.
+
+Lemma invert_pure_call `{Encode Y} f v (φ : Y -> Prop) :
+  pure (call f v) φ ⊥ ->
+  (exists η a, f = VClo η a) \/ exists η rbs g, f = VCloRec η rbs g.
+Proof.
+  intros Hcall.
+  unfold call in Hcall.
+  destruct f; simpl in Hcall;
+    ((exfalso; by eapply invert_pure_wp_crash) || eauto).
+Qed.
+
+(* -------------------------------------------------------------------------- *)
+(** *Evaluating recursive function calls *)
 (* -------------------------------------------------------------------------- *)
 
 (* A well-founded relation *)
@@ -237,6 +191,7 @@ Definition WellFoundedRel_WellFounded {A} (R : A -> A -> Prop)
 
 (* -------------------------------------------------------------------------- *)
 
+(* Recursive calls *)
 Lemma pure_rec_call `{Encode X, Encode Y} (WF_x : WellFounded X)
   (η : env) (f : var) arg e (x : X) Ψ (P : X -> Prop) (φ : X -> Y -> Prop):
   P x ->
@@ -290,7 +245,7 @@ Lemma pure_rec_call_measure_gen `{Encode X, Encode Y} {M}
   (∀ vf (y' : X),
     (∀ (y : X),
         wf_relation (WF := WF_x) (measure y) (measure y') ->
-        pure (call vf #y) (φ y) Ψ) ->
+         pure (call vf #y) (φ y) Ψ) ->
     (pure (eval ((arg, #y') :: (f, vf) :: η) e) (φ y') Ψ)) ->
     pure (call (VCloRec η [RecBinding f (AnonFun arg e)] f) #x) (φ x) Ψ.
 Proof.
@@ -304,7 +259,51 @@ Proof.
   specialize (IH _ H1). eapply IH; done.
 Qed.
 
+Lemma pure_rec_call_measure' `{Encode X, Encode Y} {M}
+  (measure : X -> M) (WF_x : WellFounded M)
+  (η : env) (f : var) arg e Ψ (φ : Y -> Prop) x P:
+  P x ->
+  (∀ vf (y' : X),
+    (∀ (y : X),
+        wf_relation (WF := WF_x) (measure y) (measure y') ->
+        (P y -> pure (call vf #y) φ Ψ)) ->
+    (pure (eval ((arg, #y') :: (f, vf) :: η) e) φ Ψ)) ->
+    pure (call (VCloRec η [RecBinding f (AnonFun arg e)] f) #x) φ Ψ.
+Proof.
+  intros HP Hrec.
+  remember (measure x). revert x HP Heqm.
+  induction m as [mx IH] using (well_founded_induction wf_def); intros.
+  simpl; rewrite String.eqb_refl.
+  apply pure_wp_bind, pure_wp_ret. simpl.
+  apply pure_CEval; rewrite try2_ret_right. subst.
+  apply Hrec. intros; subst.
+  specialize (IH _ H1). eapply IH; done.
+Qed.
+
+(* FIXME Clean up *)
+Lemma pure_rec_call_measure_gen' `{Encode X, Encode Y} {M}
+  (measure : X -> M) (WF_x : WellFounded M) x P
+  (η : env) (f : var) arg e Ψ (φ : X -> Y -> Prop):
+  P x ->
+  (∀ vf (y' : X),
+    (∀ (y : X),
+        wf_relation (WF := WF_x) (measure y) (measure y') ->
+        (P y -> pure (call vf #y) (φ y) Ψ)) ->
+    (P y' -> pure (eval ((arg, #y') :: (f, vf) :: η) e) (φ y') Ψ)) ->
+    pure (call (VCloRec η [RecBinding f (AnonFun arg e)] f) #x) (φ x) Ψ.
+Proof.
+  intros HP Hrec.
+  remember (measure x). revert x HP Heqm.
+  induction m as [mx IH] using (well_founded_induction wf_def); intros.
+  simpl; rewrite String.eqb_refl.
+  apply pure_wp_bind, pure_wp_ret. simpl.
+  apply pure_CEval; rewrite try2_ret_right. subst.
+  apply Hrec. intros; subst.
+  specialize (IH _ H1). eapply IH; done. done.
+Qed.
+
 (* Tactics for reasoning about recursive calls. *)
+(* TODO rename and comment *)
 
 Tactic Notation "recursion" constr(t) :=
   (eapply (pure_rec_call (X := t) _)).
@@ -314,14 +313,14 @@ Tactic Notation "recursion" uconstr(H) "with" uconstr(R) :=
   (eapply (pure_rec_call (WellFoundedRel_WellFounded R)) with (P := H)).
 Tactic Notation "recursion" "{" "measure " uconstr(measure) "}" "∀" uconstr(g) :=
   (eapply (pure_rec_call_measure_gen measure _ g)).
+Tactic Notation "recursion" "{" "measure " uconstr(measure) "}" "∀" uconstr(g) "gen" uconstr(P) :=
+  (eapply (pure_rec_call_measure_gen' measure _ g P)).
 Tactic Notation "recursion" "with" uconstr(R) "{" "measure " uconstr(measure) "}" :=
   (eapply (pure_rec_call_measure measure (WellFoundedRel_WellFounded R))).
 Tactic Notation "recursion" "with" uconstr(R) "{" "measure " uconstr(measure) "}" "∀" uconstr(g) :=
   (eapply (pure_rec_call_measure_gen measure (WellFoundedRel_WellFounded R) g)).
 
 (* -------------------------------------------------------------------------- *)
-
-From osiris.program_logic.pure Require Import pattern_rules.
 
 (* -------------------------------------------------------------------------- *)
 (** *Evaluating pattern matches *)
@@ -397,8 +396,6 @@ Section match_rules.
   Proof.
     intros Hpat. simpl_eval_trywith.
     eapply pure_wp_try, pure_wp_mono; eauto.
-    apply pattern_equals_pat; eauto.
-    all: intros; eauto.
   Qed.
 
   (* Currently unused *)
@@ -409,7 +406,7 @@ Section match_rules.
   Proof.
     unfold pure_match.
     intros; simpl_deep_eval_match.
-    apply pure_wp_try. by apply cpattern_equals_cpat.
+    apply pure_wp_try. eassumption.
   Qed.
 
   Lemma pure_match_cons `{Encode A} η v p e bs (φ : A -> Prop) ψ ζ :
@@ -419,13 +416,14 @@ Section match_rules.
   Proof.
     intros.
     apply pure_match_cons_unary.
-    apply cpattern_equals_cpat.
-    eapply pure_wp_mono.
-    by apply cpattern_equals_cpat.
-    all: intros; eauto.
+    by eapply pure_wp_mono.
   Qed.
 
   (* Not matching is an error. *)
+
+  Lemma pure_match_nil `{Encode A} η o (φ : A -> Prop) Ψ :
+    False -> pure_match η nil o φ Ψ.
+  Proof. contradiction. Qed.
 
   Lemma pure_match_single `{Encode A} η v p e (φ : A -> Prop) ψ ζ :
     cpattern η p v (λ η' : env, pure (eval η' e) φ ζ) ψ →
@@ -453,22 +451,38 @@ Section eval_rules.
   Lemma pure_eval_path `{Encode A} η π (ψ : A -> Prop) (ζ : exn -> Prop) :
     total (lookup_path η π) ψ ->
     pure (eval η (EPath π)) ψ ζ.
-  Proof. simpl_eval. Admitted.
+  Proof.
+    simpl_eval. apply pure_wp_widen.
+  Qed.
 
-  Lemma pure_eval_tuple `{Encode A, Encode B} η x tl (φ : B -> Prop) ψ v:
+  Lemma pure_eval_tuple `{Encode A} η hd tl (φ : val -> Prop) v:
     pure (A := A)
-      (eval η x)
+      (eval η hd)
       (fun v' : A =>
-        pure_wp (evals η tl) (fun x => v = # v' :: x) ψ) ψ ->
-    pure (A := B) (eval η (ETuple (x :: tl))) φ ψ.
-  Proof. Admitted.
+        pure_wp (evals η tl)
+          (fun x => v = # v' :: x /\ φ (VTuple (# v' :: x))) ⊥) ⊥ ->
+    pure (eval η (ETuple (hd :: tl))) φ ⊥.
+  Proof.
+    intros. simpl_eval.
+    eapply pure_wpv_Par_left_conseq; first done. intros ? (? & -> & ?).
+    eapply pure_wp_mono; try done.
+    intros * (->&?). apply pure_wp_ret.
+    eauto with pure.
+  Qed.
 
-  Lemma pure_evals_cons `{Encode A} η (hd : expr) tl (φ : list val -> Prop) ψ :
-    pure (A := A) (eval η hd)
-      (fun x =>
-        pure_wp (evals η tl) (fun v => φ (# x :: v)) ψ) ψ ->
-    pure_wp (A := list val) (evals η (hd :: tl)) φ ψ.
-  Proof. Admitted.
+  (* Lemma pure_evals_cons `{Encode A} η (hd : expr) tl (φ : list val -> Prop) ψ : *)
+  (*   pure (A := A) (eval η hd) *)
+  (*     (fun x => *)
+  (*       pure_wp (evals η tl) (fun v => φ (# x :: v)) ψ) ψ -> *)
+  (*   pure_wp (A := list val) (evals η (hd :: tl)) φ ψ. *)
+  (* Proof. *)
+  (*   intros. simpl_evals. *)
+  (*   eapply pure_wpv_Par_left_conseq; first done. intros ? (? & -> & ?). *)
+  (*   eapply pure_wp_mono; try done. *)
+  (*   intros * (->&?). apply pure_wp_ret. *)
+  (*   eauto with pure. *)
+  (* Qed. *)
+  (* Admitted. *)
 
   (* -------------------------------------------------------------------------- *)
 
@@ -480,7 +494,7 @@ Section eval_rules.
   (* Proof. *)
   (*   simpl. *)
   (*   intros He. simpl_eval. *)
-  (*   eapply pure_bind, pure_bind, (pure_mono _ He); auto. *)
+  (*   eapply pure_bind, pure_bind, (pure_wp_mono _ He); auto. *)
   (*   intros _v ([] & -> & H); apply pure_ret, H. *)
   (* Qed. *)
 
@@ -504,8 +518,8 @@ Section eval_rules.
   (*   eauto using pure_bind. *)
   (* Qed. *)
 
-  (* (* If [z] is representable and [z ≠ 0] then the runtime check *)
-  (*   performed by [check_div_by_zero (repr z)] must succeed. *) *)
+  (* (* If [z] is representable and [z ≠ 0] then the runtime check *) *)
+  (* (*   performed by [check_div_by_zero (repr z)] must succeed. *) *)
 
   (* Lemma pure_check_div_by_zero z : *)
   (*   representable z → *)
@@ -574,37 +588,14 @@ Section eval_rules.
       + intros exn []; repeat constructor; eauto.
   Qed.
 
+  Lemma pure_evals_eq η es vs ψ :
+    Forall2 (λ e v, pure (eval η e) (λ x, x = v) ψ) es vs →
+    pure (evals η es) (λ x, x = vs) ψ.
+  Proof.
+    apply pure_wp_evals_eq.
+  Qed.
+
   (* -------------------------------------------------------------------------- *)
-
-  Context {A} {EncA: Encode A}.
-
-  (** Hoare reasoning rules *)
-
-  Lemma pure_ifthenelse η e e1 e2 φ (ψ : exn -> Prop) :
-    pure (A := bool) (eval η e)
-      (λ v : bool, pure (eval η (if v then e1 else e2)) φ ψ) ψ →
-    pure (A := A) (eval η (EIfThenElse e e1 e2)) φ ψ.
-  Proof.
-    simpl.
-    intros He. simpl_eval.
-    eapply pure_wp_bind, pure_wp_bind, (pure_wp_mono _ He); eauto.
-    intros _v ([] & -> & H);
-    apply pure_wp_ret, H.
-  Qed.
-
-  Lemma pure_assert η e ψ :
-    pure (eval η e) (λ v, v = #true) ψ →
-    pure (eval η (EAssert e)) (λ v, v = #()) ψ.
-  Proof.
-    intros He. simpl_eval.
-    apply pure_choose. eapply pure_ret; eauto.
-    apply pure_wp_bind, pure_wp_bind.
-    apply (pure_wp_mono _ He); auto.
-    intros _ (?&->&->); repeat econstructor.
-  Qed.
-
-  Definition pure_call2 `{Encode X} vf arg1 arg2 (φ : X -> Prop) Ψ :=
-    pure (call vf arg1) (fun c => pure (call c arg2) (returns φ) Ψ) Ψ.
 
   (* Tuples. *)
 
@@ -623,168 +614,300 @@ Section eval_rules.
     eauto with pure.
   Qed.
 
+  Lemma pure_eval_triple `{Encode A1, Encode A2, Encode A3} η e1 e2 e3 (ψ : A1 * A2 * A3 -> Prop) :
+    pure (eval η e1) (λ a1 : A1,
+          pure (eval η e2) (λ a2 : A2,
+                pure (eval η e3) (λ a3 : A3,
+                      ψ (a1, a2, a3)) ⊥) ⊥) ⊥ ->
+    pure (eval η (ETuple [e1; e2; e3])) ψ ⊥.
+  Proof.
+    intros. simpl_eval.
+    eapply pure_wpv_Par_left_conseq; eauto. intros ? (? & -> & ?).
+    eapply pure_wpv_Par_left_conseq; eauto. intros ? (? & -> & ?).
+    eapply pure_wpv_Par_left_conseq; eauto. intros ? (? & -> & ?).
+    repeat apply pure_wp_ret.
+    eauto with pure.
+  Qed.
+
+  Lemma pure_eval_quadruple `{Encode A1, Encode A2, Encode A3, Encode A4} (η : env) (e1 e2 e3 e4 : expr)
+    (ψ : A1 * A2 * A3 * A4 → Prop) :
+    pure (eval η e1) (λ a1 : A1,
+          pure (eval η e2) (λ a2 : A2,
+                pure (eval η e3) (λ a3 : A3,
+                      pure (eval η e4) (λ a4 : A4,
+                            ψ (a1, a2, a3, a4)) ⊥) ⊥) ⊥) ⊥ ->
+    pure (eval η (ETuple [e1; e2; e3; e4])) ψ ⊥.
+  Proof.
+    intros. simpl_eval.
+    eapply pure_wpv_Par_left_conseq; eauto. intros ? (? & -> & ?).
+    eapply pure_wpv_Par_left_conseq; eauto. intros ? (? & -> & ?).
+    eapply pure_wpv_Par_left_conseq; eauto. intros ? (? & -> & ?).
+    eapply pure_wpv_Par_left_conseq; eauto. intros ? (? & -> & ?).
+    repeat apply pure_wp_ret.
+    eauto with pure.
+  Qed.
+
+  (* -------------------------------------------------------------------------- *)
+  (* Helper lemmas for operations on Booleans. *) (* TODO: Move *)
+  Lemma pure_as_bool (m : microvx) (φ : bool → Prop) ψ :
+    pure m φ ψ →
+    pure (as_bool m) φ ψ.
+  Proof.
+    intro H.
+    eapply pure_wp_bind_conseq; eauto.
+    intros [] ([] & E & Hb); discriminate || rewrite E;
+      with_strategy transparent [val_as_bool] by constructor.
+  Qed.
+  (* -------------------------------------------------------------------------- *)
+
+  (** Hoare reasoning rules *)
+
+  (* Conditionals. *)
+
+  Lemma pure_ifthenelse `{EncA: Encode A}
+    η e e1 e2 φ (ψ : exn -> Prop) :
+    pure (A := bool) (eval η e)
+      (λ v : bool, pure (eval η (if v then e1 else e2)) φ ψ) ψ →
+    pure (A := A) (eval η (EIfThenElse e e1 e2)) φ ψ.
+  Proof.
+    intros He. simpl_eval.
+    eapply pure_wp_bind, pure_wp_bind, (pure_wp_mono _ He); auto.
+    intros _v ([] & -> & H).
+    all: eapply pure_wp_simp; [ simp | ];
+    apply pure_wp_ret, H.
+  Qed.
+
+  (* TODO fix inconsistent naming *)
+  Lemma pure_ifthenelse_bool `{EncA: Encode A}
+    η e e1 e2 (φ : A -> _) φb ψ :
+    pure (eval η e) φb ψ →
+    (φb true  → pure (eval η e1) φ ψ) →
+    (φb false → pure (eval η e2) φ ψ) →
+    pure (eval η (EIfThenElse e e1 e2)) φ ψ.
+  Proof.
+    simpl.
+    intros Hb Ht Hf.
+    simpl_eval.
+    eapply pure_wp_bind_conseq. apply pure_as_bool. apply Hb.
+    intros [] ?; eauto with pure.
+  Qed.
+
+  Lemma pure_eval_ifthenelse `{EncA: Encode A}
+    η e e1 e2 (P : Prop) (ψ : A → Prop) :
+    pure (eval η e) (λ P', P' <-> P) ⊥ →
+    (P → pure (eval η e1) ψ ⊥) →
+    (~ P → pure (eval η e2) ψ ⊥) →
+    pure (eval η (EIfThenElse e e1 e2)) ψ ⊥.
+  Proof.
+    intros He He1 He2.
+    eapply pure_ifthenelse.
+    eapply (pure_wp_mono_ret _ He).
+    intros _v (_ & -> & ->%iff_encode). exists (truth P).
+    rewrite encode_truth. split; auto.
+    generalize (truth_elim P).
+    destruct (truth P); eauto.
+  Qed.
+
+  Lemma pure_assert η e ψ :
+    pure (eval η e) (λ v, v = #true) ψ →
+    pure (eval η (EAssert e)) (λ v, v = #()) ψ.
+  Proof.
+    intros He. simpl_eval.
+    apply pure_choose. eapply pure_ret; eauto.
+    apply pure_wp_bind, pure_wp_bind.
+    apply (pure_wp_mono _ He); auto.
+    intros _ (?&->&->).
+    eapply pure_wp_simp; [ simp | ];
+    repeat econstructor.
+  Qed.
+
   (* TODO: comment *)
 
-  (* Lemma total_eval_int η i (ψ : Z -> Prop) : *)
-  (*   ψ i -> *)
-  (*   total (eval η (EInt i)) ψ. *)
-  (* Proof. *)
-  (*   intros. *)
-  (*   eapply pure_wp_simp. simp_tactics.simp. *)
-  (*   eapply total_ret; eauto. *)
-  (* Qed. *)
+  Lemma total_eval_int η i (ψ : Z -> Prop) :
+    ψ i ->
+    total (eval η (EInt i)) ψ.
+  Proof.
+    intros.
+    eapply pure_wp_simp.
+    simp.
+    eapply total_ret; eauto.
+  Qed.
 
-  (* (* Function applications. *) *)
+  (* Function applications. *)
 
-  (* Lemma pure_eval_anonfun `{Encode A, Encode A1} η v e (φ : A1 -> Prop) (ψ : val -> Prop) ζ : *)
-  (*   (∀ (x : A), pure (eval ((v, #x) :: η) e) φ ζ) -> *)
-  (*   (∀ (vf : val), (∀ (x : A), pure (call vf #x) φ ζ) -> ψ vf) -> *)
-  (*   pure (eval η (EAnonFun (AnonFun v e))) ψ ζ. *)
-  (* Proof. *)
-  (*   intros Hcall Hcov. specialize (Hcov (VClo η (AnonFun v e))). *)
-  (*   eapply pure_wp_simp; [ simp | eauto ]. *)
-  (*   eapply pure_wp_ret. eexists. split. by encode. *)
-  (*   apply Hcov. *)
-  (*   intros. eapply pure_wp_simp; [ simp | apply Hcall ]. *)
-  (* Qed. *)
+  Lemma pure_eval_anonfun {A A1}
+    {EncA: Encode A} {EncA1: Encode A1}
+    η v e (φ : A1 -> Prop) (ψ : val -> Prop) ζ :
+    (∀ (x : A), pure (eval ((v, #x) :: η) e) φ ζ) ->
+    (∀ (vf : val), (∀ (x : A), pure (call vf #x) φ ζ) -> ψ vf) ->
+    pure (eval η (EAnonFun (AnonFun v e))) ψ ζ.
+  Proof.
+    intros Hcall Hcov. specialize (Hcov (VClo η (AnonFun v e))).
+    eapply pure_wp_simp; [ simp | eauto ].
+    eapply pure_wp_ret. eexists. split. by encode.
+    apply Hcov.
+    intros. eapply pure_wp_simp; [ simp | apply Hcall ].
+  Qed.
 
-  (* Lemma pure_eval_anonfun' `{Encode A, Encode A1} η a φ (ψ : val -> Prop) : *)
-  (*   (∀ (x : A), φ (VClo η a) #x) -> *)
-  (*   (∀ (vf : val), (∀ (x : A), φ vf #x) -> ψ vf) -> *)
-  (*   total (eval η (EAnonFun a)) ψ. *)
-  (* Proof. *)
-  (*   intros Hcall Hcov. specialize (Hcov (VClo η a)). *)
-  (*   eapply pure_wp_simp; [ simp | eauto ]. *)
-  (*   eapply total_ret; first solve [encode]. *)
-  (*   eauto. *)
-  (* Qed. *)
+  Lemma pure_eval_anonfun' {A A1}
+    {EncA: Encode A} {EncA1: Encode A1} η a φ (ψ : val -> Prop) :
+    (∀ (x : A), φ (VClo η a) #x) ->
+    (∀ (vf : val), (∀ (x : A), φ vf #x) -> ψ vf) ->
+    total (eval η (EAnonFun a)) ψ.
+  Proof.
+    intros Hcall Hcov. specialize (Hcov (VClo η a)).
+    eapply pure_wp_simp; [ simp | eauto ].
+    eapply total_ret; first solve [encode].
+    eauto.
+  Qed.
 
-  (* Lemma pure_eval_anonfunction `{Encode A, Encode A1} η bs (φ : A1 -> Prop) (ψ : val -> Prop) : *)
-  (*   (∀ (x : A), *)
-  (*       total *)
-  (*         (deep_eval_match (("__osiris_anonymous_arg", #x) :: η) bs (O2Ret #x)) *)
-  (*         φ) -> *)
-  (*   (∀ (vf : val), (∀ (x : A), total (call vf #x) φ) -> ψ vf) -> *)
-  (*   total (eval η (EAnonFun (AnonFunction bs))) ψ. *)
-  (* Proof. *)
-  (*   intros Hcall Hcov. *)
-  (*   eapply pure_wp_simp; [ simp | eauto ]. *)
-  (*   eapply total_ret; first solve [encode]. *)
-  (*   apply Hcov. *)
-  (*   intros. eapply pure_wp_simp; [ simp  |  ]. *)
-  (*   specialize (Hcall x); generalize Hcall; by simpl_deep_eval_match. *)
-  (* Qed. *)
+  Lemma pure_eval_anonfunction {A A1}
+    {EncA: Encode A} {EncA1: Encode A1}
+    η bs (φ : A1 -> Prop) (ψ : val -> Prop) :
+    (∀ (x : A),
+        total
+          (deep_eval_match (("__osiris_anonymous_arg", #x) :: η) bs (O2Ret #x))
+          φ) ->
+    (∀ (vf : val), (∀ (x : A), total (call vf #x) φ) -> ψ vf) ->
+    total (eval η (EAnonFun (AnonFunction bs))) ψ.
+  Proof.
+    intros Hcall Hcov.
+    eapply pure_wp_simp; [ simp | eauto ].
+    eapply total_ret; first solve [encode].
+    apply Hcov.
+    intros. eapply pure_wp_simp; [ simp  |  ].
+    specialize (Hcall x); generalize Hcall; by simpl_deep_eval_match.
+  Qed.
 
-  (* (* this sequentialized lemma create only one [pure] goal but assumes [e1] cannot *) *)
-  (* (* throw exceptions *) *)
-  (* Lemma pure_eval_app `{Encode A1, Encode A} η e1 e2 (ψ : A → Prop) ζ : *)
-  (*   pure (eval η e1) *)
-  (*     (λ f : val, *)
-  (*         pure (eval η e2) *)
-  (*           (λ arg : A1, *)
-  (*               pure (call f #arg) ψ ζ) ⊥) ⊥ → *)
-  (*   pure (eval η (EApp e1 e2)) ψ ζ. *)
-  (* Proof. *)
-  (*   intros He1. simpl_eval. *)
-  (*   apply pure_wp_Par_vals_left. *)
-  (*   eapply (pure_wp_mono_ret _ He1). intros ? (v & -> & He2). *)
-  (*   eapply (pure_wp_mono _ He2); try done. *)
-  (*   intros ? (a2 & -> & Hcall). apply Hcall. *)
-  (* Qed. *)
+  (* this sequentialized lemma create only one [pure] goal but assumes [e1] cannot *)
+  (* throw exceptions *)
+  Lemma pure_eval_app {A A1}
+    {EncA: Encode A} {EncA1:Encode A1}
+    η e1 e2 (ψ : A → Prop) ζ :
+    pure (eval η e1)
+      (λ f : val,
+          pure (eval η e2)
+            (λ arg : A1,
+                pure (call f #arg) ψ ζ) ⊥) ⊥ →
+    pure (eval η (EApp e1 e2)) ψ ζ.
+  Proof.
+    intros He1. simpl_eval.
+    apply pure_wp_Par_vals_left.
+    eapply (pure_wp_mono_ret _ He1). intros ? (v & -> & He2).
+    eapply (pure_wp_mono _ He2); try done.
+    intros ? (a2 & -> & Hcall). apply Hcall.
+  Qed.
 
-  (* Lemma pure_eval_app_conseq `{Encode A, Encode B} η e1 e2 *)
-  (*   (φ1 : val → Prop) (φ2 : A → Prop) (ψ : B → Prop) ζ *)
-  (* : *)
-  (*   pure (eval η e1) φ1 ζ → *)
-  (*   pure (eval η e2) φ2 ζ → *)
-  (*   (∀ v1 v2, φ1 v1 → φ2 v2 → pure (call v1 #v2) ψ ζ) → *)
-  (*   pure (eval η (EApp e1 e2)) ψ ζ. *)
-  (* Proof. *)
-  (*   intros He1 He2 Hp. simpl_eval. *)
-  (*   apply pure_par. *)
-  (*   - eapply (pure_mono _ He1). 2: apply pure_throw. *)
-  (*     intros ? (v1 & -> & Hv1). *)
-  (*     eapply (pure_mono _ He2). 2: apply pure_throw. *)
-  (*     intros ? (a & -> & Ha). apply Hp; eauto with encode. *)
-  (*   - eapply (pure_mono _ He2). 2: apply pure_throw. *)
-  (*     intros ? (v2 & -> & Hv2). *)
-  (*     eapply (pure_mono _ He1). 2: apply pure_throw. *)
-  (*     intros ? (a & -> & Ha). apply Hp; eauto with encode. *)
-  (* Qed. *)
+  Lemma pure_eval_app_conseq {A B}
+    {EncA: Encode A} {EncB: Encode B} η e1 e2
+    (φ1 : val → Prop) (φ2 : A → Prop) (ψ : B → Prop) ζ
+  :
+    pure (eval η e1) φ1 ζ →
+    pure (eval η e2) φ2 ζ →
+    (∀ v1 v2, φ1 v1 → φ2 v2 → pure (call v1 #v2) ψ ζ) →
+    pure (eval η (EApp e1 e2)) ψ ζ.
+  Proof.
+    intros He1 He2 Hp. simpl_eval.
+    apply pure_wp_Par.
+    - eapply pure_wp_mono; first apply He1;
+        last apply pure_wp_throw.
+      intros ? (v1 & -> & Hv1).
+      eapply pure_wp_mono; first apply He2;
+        last apply pure_wp_throw.
+      intros ? (a & -> & Ha). apply Hp; eauto with encode.
+    - eapply pure_wp_mono; first apply He2;
+        last apply pure_wp_throw.
+      intros ? (v1 & -> & Hv2).
+      eapply pure_wp_mono; first apply He1;
+        last apply pure_wp_throw.
+      intros ? (a & -> & Ha). apply Hp; eauto with encode.
+  Qed.
 
+  (* TODO : move or remove *)
+  Definition pure_call2 `{Encode X} vf arg1 arg2 (φ : X -> Prop) Ψ :=
+    pure (call vf arg1) (fun c => pure (call c arg2) φ Ψ) Ψ.
 
-  (* Lemma pure_eval_app2 `{Encode A, Encode B, Encode C} η e1 e2 e3 vf *)
-  (*   (arg1 : A) (arg2 : B) (ψ : C → Prop) ζ *)
-  (*   : *)
-  (*   total (eval η e1) (λ vf', vf' = vf) -> *)
-  (*   total (eval η e2) (λ arg1', arg1' = arg1) -> *)
-  (*   total (eval η e3) (λ arg2', arg2' = arg2) -> *)
-  (*   pure_call2 vf #arg1 #arg2 ψ ζ -> *)
-  (*   pure (eval η (EApp (EApp e1 e2) e3)) ψ ζ. *)
-  (* Proof. *)
-  (*   intros He1 He2 He3 Hcall. *)
-  (*   eapply pure_simp; [ simp | eauto ]. *)
-  (*   apply pure_Par_val_right. *)
-  (*   apply (pure_mono_ret _ He3). intros ? (? & -> & ->). *)
-  (*   apply pure_Par_vals_left. *)
-  (*   apply (pure_mono_ret _ He1). intros ? (? & -> & <-). *)
-  (*   apply (pure_mono_ret _ He2). intros ? (? & -> & ->). *)
-  (*   unfold continue. simpl. *)
-  (*   apply (pure_mono _ Hcall). auto. *)
-  (*   intros ??; unfold discontinue; simpl; auto using pure_throw. *)
-  (* Qed. *)
+  Lemma pure_eval_app2 `{Encode A, Encode B, Encode C}
+    η e1 e2 e3 vf
+    (arg1 : A) (arg2 : B) (ψ : C → Prop) ζ
+    :
+    total (eval η e1) (λ vf', vf' = vf) ->
+    total (eval η e2) (λ arg1', arg1' = arg1) ->
+    total (eval η e3) (λ arg2', arg2' = arg2) ->
+    pure_call2 vf #arg1 #arg2 ψ ζ ->
+    pure (eval η (EApp (EApp e1 e2) e3)) ψ ζ.
+  Proof.
+    intros He1 He2 He3 Hcall.
+    eapply pure_wp_simp; [ simp | eauto ].
+    apply pure_wp_Par_val_right.
+    apply (pure_wp_mono_ret _ He3). intros ? (? & -> & ->).
+    apply pure_wp_Par_vals_left.
+    apply (pure_wp_mono_ret _ He1). intros ? (? & -> & <-).
+    apply (pure_wp_mono_ret _ He2). intros ? (? & -> & ->).
+    unfold continue. simpl.
+    apply (pure_wp_mono _ Hcall). auto.
+    intros ? (?&?&?); unfold discontinue; subst; simpl.
+    eapply pure_wp_mono; first apply H3; eauto.
+    intros; cbn; auto using pure_wp_throw.
+  Qed.
 
-  (* Lemma pure_eval_app2_conseq `{Encode A, Encode B, Encode C} η e1 e2 e3 vf *)
-  (*   (arg1 : A) (arg2 : B) (φ ψ : C → Prop) ζ *)
-  (*   : *)
-  (*   total (eval η e1) (λ vf', vf' = vf) -> *)
-  (*   total (eval η e2) (λ arg1', arg1' = arg1) -> *)
-  (*   total (eval η e3) (λ arg2', arg2' = arg2) -> *)
-  (*   pure_call2 vf #arg1 #arg2 φ ζ -> *)
-  (*   (∀ a, φ a → ψ a) → *)
-  (*   wp (eval η (EApp (EApp e1 e2) e3)) ψ ζ. *)
-  (* Proof. *)
-  (*   intros. *)
-  (*   eapply pure_eval_app2; eauto. *)
-  (*   eapply pure_mono; first eassumption; last auto. *)
-  (*   simpl; intros. *)
-  (*   eapply total_consequence; eauto. *)
-  (* Qed. *)
+  Lemma pure_eval_app2_conseq `{Encode A, Encode B, Encode C}
+    η e1 e2 e3 vf
+    (arg1 : A) (arg2 : B) (φ ψ : C → Prop) ζ
+    :
+    total (eval η e1) (λ vf', vf' = vf) ->
+    total (eval η e2) (λ arg1', arg1' = arg1) ->
+    total (eval η e3) (λ arg2', arg2' = arg2) ->
+    pure_call2 vf #arg1 #arg2 φ ζ ->
+    (∀ a, φ a → ψ a) →
+    pure (eval η (EApp (EApp e1 e2) e3)) ψ ζ.
+  Proof.
+    intros.
+    eapply pure_eval_app2; eauto.
+    eapply pure_mono; first eassumption; last auto.
+    simpl; intros.
+    eapply pure_mono; eauto.
+  Qed.
 
   (* Helper lemmas for arithmetic operations. *)
 
-  (* Lemma pure_as_int m (φ : Z → Prop) : *)
-  (*   total m φ → *)
-  (*   total (as_int m) (λ i, ∃ z, i = repr z ∧ φ z). *)
+  (* Lemma pure_as_int {A} m (φ : Z → Prop) ψ: *)
+  (*   pure m φ ψ → *)
+  (*   pure (E := exn) (as_int m) *)
+  (*     (λ i, ∃ z, i = repr z ∧ φ z) ⊥. *)
   (* Proof. *)
-  (*   intros Hm. apply pure_bind. *)
-  (*   apply (pure_mono_ret _ Hm). intros ? (z & -> & Hz). *)
-  (*   apply pure_ret. eauto. *)
+  (*   intros Hm. *)
+  (*   apply (pure_wp_mono_ret _ Hm). intros ? (z & -> & Hz). *)
+  (*   econstructor; split; eauto. cbn. *)
+  (*   repeat f_equiv. Search M.intval repr.  re *)
+  (*   econstructor; split; eauto. cbn. *)
+  (*   eauto with pure. apply pure_wp_ret. eauto. *)
   (* Qed. *)
 
   (* Lemma pure_enc_par_as_int m1 m2 (φ1 φ2 φ : Z → Prop) k : *)
-  (*   pure m1 ##φ1 ⊥ → *)
-  (*   pure m2 ##φ2 ⊥ → *)
-  (*   (∀ z1 z2 : Z, φ1 z1 → φ2 z2 → pure (k (repr z1, repr z2)) ##φ ⊥) → *)
-  (*   pure (Par (as_int m1) (as_int m2) (pfbind inject2 k)) ##φ ⊥. *)
+  (*   pure m1 φ1 ⊥ → *)
+  (*   pure m2 φ2 ⊥ → *)
+  (*   (∀ z1 z2 : Z, φ1 z1 → φ2 z2 → pure (k (repr z1, repr z2)) φ ⊥) → *)
+  (*   pure (Par (as_int m1) (as_int m2) (pfbind inject2 k)) φ ⊥. *)
   (* Proof. *)
   (*   intros Hm1 Hm2 Hk. *)
   (*   unfold as_int. *)
-  (*   eapply pure_Par_conseq. 1,2: eapply pure_as_int; eauto. 2: firstorder. *)
+  (*   eapply pure_wp_Par_conseq. 1,2: eapply pure_as_int; eauto. 2: firstorder. *)
   (*   intros ? ? (z1 & -> & Hz1) (z2 & -> & Hz2). *)
   (*   eapply pure_simp; [ simp | ]. *)
   (*   by apply Hk. *)
   (* Qed. *)
 
-  (* (* Primitive arithmetic operations. *) *)
+  (* Primitive arithmetic operations. *)
 
   (* Lemma pure_eval_add η e1 e2 (φ1 φ2 φ : Z → Prop) : *)
-  (*   pure (eval η e1) ##φ1 ⊥ → *)
-  (*   pure (eval η e2) ##φ2 ⊥ → *)
+  (*   pure (eval η e1) φ1 ⊥ → *)
+  (*   pure (eval η e2) φ2 ⊥ → *)
   (*   (∀ z1 z2, φ1 z1 → φ2 z2 → φ (z1 + z2)) → *)
-  (*   pure (eval η (EIntAdd e1 e2)) ##φ ⊥. *)
+  (*   pure (eval η (EIntAdd e1 e2)) φ ⊥. *)
   (* Proof. *)
-  (*   intros. simpl_eval. eapply pure_enc_par_as_int; eauto. intros. *)
+  (*   intros. simpl_eval. *)
+  (*   eapply pure_enc_par_as_int; eauto. intros. *)
   (*   eapply pure_enc_ret; eauto with encode. *)
   (* Qed. *)
 
@@ -825,7 +948,7 @@ Section eval_rules.
   (*   eauto 10 with encode. *)
   (* Qed. *)
 
-  (* (* Primitive logical operations on machine integers. *) *)
+  (* Primitive logical operations on machine integers. *)
 
   (* Lemma pure_eval_lnot η e1 (φ1 φ : Z → Prop) : *)
   (*   pure (eval η e1) ##φ1 ⊥ → *)
@@ -906,485 +1029,430 @@ Section eval_rules.
   (*   eapply pure_enc_ret; eauto with encode. *)
   (* Qed. *)
 
-  (* (* Helper lemmas for operations on Booleans. *) *)
-
-  (* Lemma pure_as_bool (m : microvx) (φ : bool → Prop) ψ : *)
-  (*   pure m ##φ ψ → *)
-  (*   pure (as_bool m) φ ψ. *)
-  (* Proof. *)
-  (*   intro H. *)
-  (*   eapply pure_bind_conseq; eauto. *)
-  (*   intros [] ([] & E & Hb); discriminate || rewrite E; with_strategy transparent [val_as_bool] by constructor. *)
-  (* Qed. *)
-
-  (* Lemma pure_enc_bind_as_bool {A} m (φ : bool → Prop) (ψ : A → Prop) (k : bool → micro A exn) : *)
-  (*   pure m ##φ ⊥ → *)
+  (* Lemma pure_enc_bind_as_bool {A} {EncA: Encode A} m (φ : bool → Prop) (ψ : A → Prop) (k : bool → micro A exn) : *)
+  (*   pure m φ ⊥ → *)
   (*   (∀ b : bool, φ b → pure (k b) ψ ⊥) → *)
   (*   pure (bind (as_bool m) k) ψ ⊥. *)
   (* Proof. *)
-  (*   intros Hm Hp. apply pure_bind, pure_as_bool. *)
-  (*   apply (pure_mono_ret _ Hm). intros ? (b & -> & Hb). *)
-  (*   destruct b; force_unfold val_as_bool; unfold encode_pred; eauto. *)
+  (*   intros Hm Hp. apply pure_wp_bind, pure_as_bool. *)
+  (*   apply (pure_wp_mono_ret _ Hm). intros ? (b & -> & Hb). *)
+  (*   destruct b; force_unfold val_as_bool; eauto with pure. *)
   (* Qed. *)
 
-  (* (* Primitive operations on Booleans. *) *)
+  (* Primitive operations on Booleans. *)
 
   (* Lemma pure_eval_negb η e (φ ψ : bool → Prop) : *)
-  (*   pure (eval η e) ##φ ⊥ → *)
+  (*   pure (eval η e) φ ⊥ → *)
   (*   (∀ b, φ b → ψ (negb b)) → *)
-  (*   pure (eval η (EBoolNeg e)) ##ψ ⊥. *)
+  (*   pure (eval η (EBoolNeg e)) ψ ⊥. *)
   (* Proof. *)
   (*   intros He Hp. simpl_eval. *)
-  (*   eapply pure_enc_bind_as_bool; eauto. intros b Hb. apply pure_ret. eauto with encode. *)
+  (*   eapply pure_enc_bind_as_bool; eauto. intros b Hb. apply pure_wp_ret. *)
+  (*   eauto with pure. *)
   (* Qed. *)
 
   (* Lemma pure_eval_not η e (φ ψ : Prop → Prop) : *)
-  (*   pure (eval η e) ##φ ⊥ → *)
+  (*   pure (eval η e) φ ⊥ → *)
   (*   (∀ P, φ P → ψ (¬P)) → *)
-  (*   pure (eval η (EBoolNeg e)) ##ψ ⊥. *)
+  (*   pure (eval η (EBoolNeg e)) ψ ⊥. *)
   (* Proof. *)
   (*   intros He Hp. simpl_eval. *)
-  (*   eapply pure_bind. *)
+  (*   eapply pure_wp_bind. *)
   (*   eapply pure_as_bool. *)
-  (*   eapply pure_mono_ret. apply He. intros ? (P & -> & HP). *)
-  (*   exists (truth P). split; auto. apply pure_ret. eexists. split; eauto with encode. *)
+  (*   eapply pure_wp_mono_ret. apply He. intros ? (P & -> & HP). *)
+  (*   exists (truth P). split; auto. apply pure_wp_ret. eexists. split; eauto with pure. *)
   (*   unfold encode, Encode_Prop. rewrite truth_neg. auto. *)
   (* Qed. *)
 
-  (* (* Local definitions. *) *)
+  (* Local definitions. *)
 
-  (* (* TODO only one or two bindings, for now *) *)
+  (* TODO only one or two bindings, for now *)
 
-  (* (* TODO: lemmas starting with "_" are unused: remove? *) *)
+  (* TODO: lemmas starting with "_" are unused: remove? *)
 
-  (* Lemma pure_eval_let_pair `{Encode A1, Encode A2} `{Encode X} *)
-  (*   p1 p2 e1 e2 η (ψ : X -> Prop) : *)
-  (*   pure (eval η e1) ##(λ '((v1, v2) : A1 * A2), *)
-  (*       pure ( *)
-  (*           δ ← widen (irrefutably_extend [] p1 #v1); *)
-  (*           θ ← widen (irrefutably_extend δ p2 #v2); *)
-  (*           eval (θ ++ η) e2 *)
-  (*         ) ##ψ ⊥) ⊥ -> *)
-  (*   pure (eval η (ELet1 (PPair p1 p2) e1 e2)) ##ψ ⊥. *)
-  (* Proof. *)
-  (*   (* This proof is a long rewriting sequence, which makes some sense as it is *) *)
-  (* (*   not the standard method to prove a let binding, but rather a way to reduce the *) *)
-  (* (*   wp of a parallel pair to ordered wps of two binds with error handling *) *)
-  (*   intros He1. *)
-  (*   simpl_eval. apply pure_Par_vals_left. *)
-  (*   apply (pure_mono_ret _ He1). clear He1. *)
-  (*   intros ? ([v1 v2] & -> & Hpure). apply pure_ret. *)
-  (*   apply pure_bind. *)
-  (*   apply pure_bind. *)
-  (*   apply pure_ret. *)
-  (*   unfold widen, irrefutably_extend in *. *)
-  (*   rewrite !try_try in *. simpl_extend. *)
-  (*   rewrite !bind_as_try, !try_try in *. *)
-  (*   apply pure_try2. *)
-  (*   apply invert_pure_try2 in Hpure. *)
-  (*   apply (pure_mono _ Hpure); clear Hpure. *)
-  (*   - intros δ Hpure. *)
-  (*     unfold continue in *. *)
-  (*     unfold glue2 in *. *)
-  (*     repeat rewrite ?bind_as_try, ?try_try, ?try_ret in *. *)
-  (*     apply invert_pure_try2 in Hpure. *)
-  (*     apply pure_try2. *)
-  (*     apply (pure_mono _ Hpure); clear Hpure. *)
-  (*     + intros θ Hpure. *)
-  (*       unfold continue, glue2 in *. *)
-  (*       repeat rewrite ?bind_as_try, ?try_try, ?try_ret in *. *)
-  (*       apply pure_ret. eauto. *)
-  (*     + unfold match_failure. rewrite try_crash. intros. edestruct @invert_pure_crash; eauto. *)
-  (*   - unfold match_failure. rewrite try_crash. intros. edestruct @invert_pure_crash; eauto. *)
-  (* Qed. *)
+  Lemma pure_eval_let_pair `{Encode A1, Encode A2} `{Encode X}
+    p1 p2 e1 e2 η (ψ : X -> Prop) :
+    pure (eval η e1) (λ '((v1, v2) : A1 * A2),
+        pure (
+            δ ← widen (irrefutably_extend [] p1 #v1);
+            θ ← widen (irrefutably_extend δ p2 #v2);
+            eval (θ ++ η) e2
+          ) ψ ⊥) ⊥ ->
+    pure (eval η (ELet1 (PPair p1 p2) e1 e2)) ψ ⊥.
+  Proof.
+    (* This proof is a long rewriting sequence, which makes some sense as it is *)
+  (*   not the standard method to prove a let binding, but rather a way to reduce the *)
+  (*   wp of a parallel pair to ordered wps of two binds with error handling *)
+    intros He1.
+    simpl_eval. apply pure_wp_Par_vals_left.
+    apply (pure_wp_mono_ret _ He1). clear He1.
+    intros ? ([v1 v2] & -> & Hpure). apply pure_wp_ret.
+    apply pure_wp_bind.
+    apply pure_wp_bind.
+    apply pure_wp_ret.
+    unfold widen, irrefutably_extend in *.
+    rewrite !try_try in *. simpl_extend.
+    rewrite !bind_as_try, !try_try in *.
+    apply pure_wp_try2.
+    apply invert_pure_wp_try2 in Hpure.
+    apply (pure_wp_mono _ Hpure); clear Hpure.
+    - intros δ Hpure.
+      unfold continue in *.
+      unfold glue2 in *.
+      repeat rewrite ?bind_as_try, ?try_try, ?try_ret in *.
+      apply invert_pure_wp_try2 in Hpure.
+      apply pure_wp_try2.
+      apply (pure_wp_mono _ Hpure); clear Hpure.
+      + intros θ Hpure.
+        unfold continue, glue2 in *.
+        repeat rewrite ?bind_as_try, ?try_try, ?try_ret in *.
+        apply pure_wp_ret. eauto.
+      + unfold match_failure. rewrite try_crash. intros. edestruct @invert_pure_wp_crash; eauto.
+    - unfold match_failure. rewrite try_crash. intros. edestruct @invert_pure_wp_crash; eauto.
+  Qed.
 
-  (* Lemma pure_eval_let `{Encode A1, Encode B} η x e1 e *)
-  (*   (φ1 : A1 → Prop) (ψ : B → Prop) : *)
-  (*   pure (eval η e1) ##φ1 ⊥ → *)
-  (*   (∀ a1, φ1 a1 → pure (eval ((x, #a1) :: η) e) ##ψ ⊥) → *)
-  (*   pure (eval η (ELet1Var x e1 e)) ##ψ ⊥. *)
-  (* Proof. *)
-  (*   intros He1 He. *)
-  (*   simpl_eval. *)
-  (*   eapply pure_Par_conseq_ret. *)
-  (*   - eauto. *)
-  (*   - eapply pure_simp. simp. apply pure_ret_eq. *)
-  (*   - intros _v _η (a1 & -> & Ha1) ->. *)
-  (*     apply pure_bind, pure_bind, pure_ret. *)
-  (*     unfold irrefutably_extend. *)
-  (*     apply pure_widen. *)
-  (*     simpl_extend. *)
-  (*     apply pure_try, pure_ret, pure_ret, He, Ha1. *)
-  (* Qed. *)
+  Lemma pure_eval_let `{Encode A1, Encode B} η x e1 e
+    (φ1 : A1 → Prop) (ψ : B → Prop) :
+    pure (eval η e1) φ1 ⊥ →
+    (∀ a1, φ1 a1 → pure (eval ((x, #a1) :: η) e) ψ ⊥) →
+    pure (eval η (ELet1Var x e1 e)) ψ ⊥.
+  Proof.
+    intros He1 He.
+    simpl_eval.
+    eapply pure_wp_Par_conseq_ret.
+    - eauto.
+    - eapply pure_wp_simp. simp. apply pure_wp_ret_eq.
+    - intros _v _η (a1 & -> & Ha1) ->.
+      apply pure_wp_bind, pure_wp_bind, pure_wp_ret.
+      unfold irrefutably_extend.
+      apply pure_wp_widen.
+      simpl_extend.
+      apply pure_wp_try, pure_wp_ret, pure_wp_ret, He, Ha1.
+  Qed.
 
-  (* Lemma pure_eval_let' `{Encode A1, Encode B} η x e1 e *)
-  (*   (a1 : A1) (ψ : B → Prop) : *)
-  (*   pure (eval η e1) ##(λ x, x = a1) ⊥ → *)
-  (*   pure (eval ((x, #a1) :: η) e) ##ψ ⊥ → *)
-  (*   pure (eval η (ELet1Var x e1 e)) ##ψ ⊥. *)
-  (* Proof. *)
-  (*   intros He1 He2. *)
-  (*   eapply pure_eval_let; eauto. *)
-  (*   congruence. *)
-  (* Qed. *)
+  Lemma pure_eval_let' `{Encode A1, Encode B} η x e1 e
+    (a1 : A1) (ψ : B → Prop) :
+    pure (eval η e1) (λ x, x = a1) ⊥ →
+    pure (eval ((x, #a1) :: η) e) ψ ⊥ →
+    pure (eval η (ELet1Var x e1 e)) ψ ⊥.
+  Proof.
+    intros He1 He2.
+    eapply pure_eval_let; eauto.
+    congruence.
+  Qed.
 
-  (* (* Conditionals. *) *)
+  (* Helper lemma for Boolean operations *)
 
-  (* (* TODO fix inconsistent naming *) *)
-  (* Lemma pure_ifthenelse_bool η e e1 e2 φ φb ψ : *)
-  (*   pure (eval η e) ##φb ψ → *)
-  (*   (φb true  → pure (eval η e1) φ ψ) → *)
-  (*   (φb false → pure (eval η e2) φ ψ) → *)
-  (*   pure (eval η (EIfThenElse e e1 e2)) φ ψ. *)
-  (* Proof. *)
-  (*   simpl. *)
-  (*   intros Hb Ht Hf. *)
-  (*   simpl_eval. *)
-  (*   eapply pure_bind_conseq. apply pure_as_bool. apply Hb. *)
-  (*   intros []; auto. *)
-  (* Qed. *)
+  Lemma pure_eval_comparison_operator `{Encode A}
+    η e1 e2 (x1 x2 : Z) (f : val → val → micro bool exn) b a (φ : A → Prop) :
+    pure (eval η e1) (λ x1' : Z, x1' = x1) ⊥ →
+    pure (eval η e2) (λ x2' : Z, x2' = x2) ⊥ →
+    f #x1 #x2 = ret b →
+    #a = #b →
+    φ a →
+    pure (Par (eval η e1) (eval η e2) (pfbind inject2 (λ '(v1, v2), 'b ← f v1 v2; ret (VBool b)))) φ ⊥.
+  Proof.
+    intros He1 He2 Ef Ea Ha.
+    eapply pure_wp_Par_conseq_ret; eauto.
+    intros _ _ (_ & -> & ->) (_ & -> & ->).
+    apply pure_wp_bind, pure_wp_ret, pure_wp_bind.
+    rewrite Ef.
+    apply pure_wp_ret, pure_wp_ret.
+    eauto with pure.
+  Qed.
 
-  (* Lemma pure_eval_ifthenelse_bool `{Encode A} η e e1 e2 (φ : bool → Prop) (ψ : A → Prop) : *)
-  (*   pure (eval η e) ##φ ⊥ → *)
-  (*   (φ true  → pure (eval η e1) ##ψ ⊥) → *)
-  (*   (φ false → pure (eval η e2) ##ψ ⊥) → *)
-  (*   pure (eval η (EIfThenElse e e1 e2)) ##ψ ⊥. *)
-  (* Proof. *)
-  (*   intros. eapply pure_ifthenelse_bool; eauto. *)
-  (* Qed. *)
+  (* Boolean operations *)
 
-  (* Lemma pure_eval_ifthenelse `{Encode A} η e e1 e2 (P : Prop) (ψ : A → Prop) : *)
-  (*   pure (eval η e) ##(λ P', P' <-> P) ⊥ → *)
-  (*   (P → pure (eval η e1) ##ψ ⊥) → *)
-  (*   (~ P → pure (eval η e2) ##ψ ⊥) → *)
-  (*   pure (eval η (EIfThenElse e e1 e2)) ##ψ ⊥. *)
-  (* Proof. *)
-  (*   intros He He1 He2. *)
-  (*   eapply pure_ifthenelse. *)
-  (*   eapply (pure_mono_ret _ He). *)
-  (*   intros _v (_ & -> & ->%iff_encode). exists (truth P). *)
-  (*   rewrite encode_truth. split; auto. *)
-  (*   generalize (truth_elim P). *)
-  (*   destruct (truth P); auto. *)
-  (* Qed. *)
+  Lemma pure_eval_EOpLe η e1 e2 (x1 x2 : Z) :
+    pure (eval η e1) (λ x1', x1' = x1) ⊥ ->
+    pure (eval η e2) (λ x2', x2' = x2) ⊥ ->
+    (* Representability hypotheses last for [x1] and [x2] evar initialisation *)
+    representable x1 ->
+    representable x2 ->
+    pure (eval η (EOpLe e1 e2)) (λ P, P <-> (x1 <= x2)%Z) ⊥.
+  Proof.
+    intros He1 He2 Hx1 Hx2. simpl_eval.
+    eapply pure_eval_comparison_operator; eauto.
+    rewrite lt_repr_repr; auto.
+    simpl. f_equal. f_equal. apply truth_eq_true. lia.
+  Qed.
 
-  (* (* Helper lemma for Boolean operations *) *)
+  Lemma pure_eval_EOpLe_bool η e1 e2 (x1 x2 : Z) :
+    pure (eval η e1) (λ x1', x1' = x1) ⊥ ->
+    pure (eval η e2) (λ x2', x2' = x2) ⊥ ->
+    representable x1 ->
+    representable x2 ->
+    pure (eval η (EOpLe e1 e2)) (λ (b : bool), b <-> (x1 <= x2)) ⊥.
+  Proof.
+    intros. eapply pure_wp_mono_ret. eapply pure_eval_EOpLe; eauto.
+    intros _ (P & -> & HP). exists (truth P). by rewrite <-HP, encode_truth, Is_true_truth.
+  Qed.
 
-  (* Lemma pure_eval_comparison_operator `{Encode A} η e1 e2 (x1 x2 : Z) (f : val → val → micro bool exn) b a (φ : A → Prop) : *)
-  (*   pure (eval η e1) ##(λ x1' : Z, x1' = x1) ⊥ → *)
-  (*   pure (eval η e2) ##(λ x2' : Z, x2' = x2) ⊥ → *)
-  (*   f #x1 #x2 = ret b → *)
-  (*   #a = #b → *)
-  (*   φ a → *)
-  (*   pure (Par (eval η e1) (eval η e2) (pfbind inject2 (λ '(v1, v2), 'b ← f v1 v2; ret (VBool b)))) ##φ ⊥. *)
-  (* Proof. *)
-  (*   intros He1 He2 Ef Ea Ha. *)
-  (*   eapply pure_Par_conseq_ret; eauto. *)
-  (*   intros _ _ (_ & -> & ->) (_ & -> & ->). *)
-  (*   apply pure_bind, pure_ret, pure_bind. *)
-  (*   rewrite Ef. *)
-  (*   apply pure_ret, pure_ret. *)
-  (*   eauto with encode. *)
-  (* Qed. *)
+  Lemma pure_eval_EOpLt η e1 e2 (x1 x2 : Z) :
+    pure (eval η e1) (λ x1', x1' = x1) ⊥ ->
+    pure (eval η e2) (λ x2', x2' = x2) ⊥ ->
+    (* Representability hypotheses last for [x1] and [x2] evar initialisation *)
+    representable x1 ->
+    representable x2 ->
+    pure (eval η (EOpLt e1 e2)) (λ P, P <-> (x1 < x2)%Z) ⊥.
+  Proof.
+    intros He1 He2 Hx1 Hx2. simpl_eval.
+    eapply pure_eval_comparison_operator; eauto.
+    rewrite lt_repr_repr; auto.
+    simpl. f_equal. f_equal. apply truth_eq_true. lia.
+  Qed.
 
-  (* (* Boolean operations *) *)
+  Lemma pure_eval_EOpLt_bool η e1 e2 (x1 x2 : Z) :
+    pure (eval η e1) (λ x1', x1' = x1) ⊥ ->
+    pure (eval η e2) (λ x2', x2' = x2) ⊥ ->
+    (* Representability hypotheses last for [x1] and [x2] evar initialisation *)
+    representable x1 ->
+    representable x2 ->
+    pure (eval η (EOpLt e1 e2)) (λ (b : bool), b <-> (x1 < x2)) ⊥.
+  Proof.
+    intros. eapply pure_wp_mono_ret. eapply pure_eval_EOpLt; eauto.
+    intros _ (P & -> & HP). exists (truth P). by rewrite <-HP, encode_truth, Is_true_truth.
+  Qed.
 
-  (* Lemma pure_eval_EOpLe η e1 e2 (x1 x2 : Z) : *)
-  (*   pure (eval η e1) ##(λ x1', x1' = x1) ⊥ -> *)
-  (*   pure (eval η e2) ##(λ x2', x2' = x2) ⊥ -> *)
-  (*   (* Representability hypotheses last for [x1] and [x2] evar initialisation *) *)
-  (*   representable x1 -> *)
-  (*   representable x2 -> *)
-  (*   pure (eval η (EOpLe e1 e2)) ##(λ P, P <-> (x1 <= x2)%Z) ⊥. *)
-  (* Proof. *)
-  (*   intros He1 He2 Hx1 Hx2. simpl_eval. *)
-  (*   eapply pure_eval_comparison_operator; eauto. *)
-  (*   rewrite lt_repr_repr; auto. *)
-  (*   simpl. f_equal. f_equal. apply truth_eq_true. lia. *)
-  (* Qed. *)
+  Lemma pure_eval_EOpGt η e1 e2 (x1 x2 : Z) :
+    pure (eval η e1) (λ x1', x1' = x1) ⊥ ->
+    pure (eval η e2) (λ x2', x2' = x2) ⊥ ->
+    (* Representability hypotheses last for [x1] and [x2] evar initialisation *)
+    representable x1 ->
+    representable x2 ->
+    pure (eval η (EOpGt e1 e2)) (λ P, P <-> (x1 > x2)%Z) ⊥.
+  Proof.
+    intros He1 He2 Hx1 Hx2. simpl_eval.
+    eapply pure_eval_comparison_operator; eauto.
+    rewrite lt_repr_repr; auto.
+    simpl. f_equal. f_equal. apply truth_eq_true. lia.
+  Qed.
 
-  (* Lemma pure_eval_EOpLe_bool η e1 e2 (x1 x2 : Z) : *)
-  (*   pure (eval η e1) ##(λ x1', x1' = x1) ⊥ -> *)
-  (*   pure (eval η e2) ##(λ x2', x2' = x2) ⊥ -> *)
-  (*   representable x1 -> *)
-  (*   representable x2 -> *)
-  (*   pure (eval η (EOpLe e1 e2)) ##(λ (b : bool), b <-> (x1 <= x2)) ⊥. *)
-  (* Proof. *)
-  (*   intros. eapply pure_mono_ret. eapply pure_eval_EOpLe; eauto. *)
-  (*   intros _ (P & -> & HP). exists (truth P). by rewrite <-HP, encode_truth, Is_true_truth. *)
-  (* Qed. *)
+  Lemma pure_eval_EOpGt_bool η e1 e2 (x1 x2 : Z) :
+    pure (eval η e1) (λ x1', x1' = x1) ⊥ ->
+    pure (eval η e2) (λ x2', x2' = x2) ⊥ ->
+    (* Representability hypotheses last for [x1] and [x2] evar initialisation *)
+    representable x1 ->
+    representable x2 ->
+    pure (eval η (EOpGt e1 e2)) (λ (b : bool), b <-> (x1 > x2)) ⊥.
+  Proof.
+    intros. eapply pure_wp_mono_ret. eapply pure_eval_EOpGt; eauto.
+    intros _ (P & -> & HP). exists (truth P). by rewrite <-HP, encode_truth, Is_true_truth.
+  Qed.
 
-  (* Lemma pure_eval_EOpLt η e1 e2 (x1 x2 : Z) : *)
-  (*   pure (eval η e1) ##(λ x1', x1' = x1) ⊥ -> *)
-  (*   pure (eval η e2) ##(λ x2', x2' = x2) ⊥ -> *)
-  (*   (* Representability hypotheses last for [x1] and [x2] evar initialisation *) *)
-  (*   representable x1 -> *)
-  (*   representable x2 -> *)
-  (*   pure (eval η (EOpLt e1 e2)) ##(λ P, P <-> (x1 < x2)%Z) ⊥. *)
-  (* Proof. *)
-  (*   intros He1 He2 Hx1 Hx2. simpl_eval. *)
-  (*   eapply pure_eval_comparison_operator; eauto. *)
-  (*   rewrite lt_repr_repr; auto. *)
-  (*   simpl. f_equal. f_equal. apply truth_eq_true. lia. *)
-  (* Qed. *)
+  Lemma pure_eval_EOpGe η e1 e2 (x1 x2 : Z) :
+    pure (eval η e1) (λ x1', x1' = x1) ⊥ ->
+    pure (eval η e2) (λ x2', x2' = x2) ⊥ ->
+    (* Representability hypotheses last for [x1] and [x2] evar initialisation *)
+    representable x1 ->
+    representable x2 ->
+    pure (eval η (EOpGe e1 e2)) (λ P, P <-> (x1 >= x2)%Z) ⊥.
+  Proof.
+    intros He1 He2 Hx1 Hx2. simpl_eval.
+    eapply pure_eval_comparison_operator; eauto.
+    rewrite lt_repr_repr; auto.
+    simpl. f_equal. f_equal. apply truth_eq_true. lia.
+  Qed.
 
-  (* Lemma pure_eval_EOpLt_bool η e1 e2 (x1 x2 : Z) : *)
-  (*   pure (eval η e1) ##(λ x1', x1' = x1) ⊥ -> *)
-  (*   pure (eval η e2) ##(λ x2', x2' = x2) ⊥ -> *)
-  (*   (* Representability hypotheses last for [x1] and [x2] evar initialisation *) *)
-  (*   representable x1 -> *)
-  (*   representable x2 -> *)
-  (*   pure (eval η (EOpLt e1 e2)) ##(λ (b : bool), b <-> (x1 < x2)) ⊥. *)
-  (* Proof. *)
-  (*   intros. eapply pure_mono_ret. eapply pure_eval_EOpLt; eauto. *)
-  (*   intros _ (P & -> & HP). exists (truth P). by rewrite <-HP, encode_truth, Is_true_truth. *)
-  (* Qed. *)
+  Lemma pure_eval_EOpGe_bool η e1 e2 (x1 x2 : Z) :
+    pure (eval η e1) (λ x1', x1' = x1) ⊥ ->
+    pure (eval η e2) (λ x2', x2' = x2) ⊥ ->
+    (* Representability hypotheses last for [x1] and [x2] evar initialisation *)
+    representable x1 ->
+    representable x2 ->
+    pure (eval η (EOpGe e1 e2)) (λ (b : bool), b <-> (x1 >= x2)) ⊥.
+  Proof.
+    intros. eapply pure_wp_mono_ret. eapply pure_eval_EOpGe; eauto.
+    intros _ (P & -> & HP). exists (truth P). by rewrite <-HP, encode_truth, Is_true_truth.
+  Qed.
 
-  (* Lemma pure_eval_EOpGt η e1 e2 (x1 x2 : Z) : *)
-  (*   pure (eval η e1) ##(λ x1', x1' = x1) ⊥ -> *)
-  (*   pure (eval η e2) ##(λ x2', x2' = x2) ⊥ -> *)
-  (*   (* Representability hypotheses last for [x1] and [x2] evar initialisation *) *)
-  (*   representable x1 -> *)
-  (*   representable x2 -> *)
-  (*   pure (eval η (EOpGt e1 e2)) ##(λ P, P <-> (x1 > x2)%Z) ⊥. *)
-  (* Proof. *)
-  (*   intros He1 He2 Hx1 Hx2. simpl_eval. *)
-  (*   eapply pure_eval_comparison_operator; eauto. *)
-  (*   rewrite lt_repr_repr; auto. *)
-  (*   simpl. f_equal. f_equal. apply truth_eq_true. lia. *)
-  (* Qed. *)
+  Lemma pure_eval_EOpEq η e1 e2 (x1 x2 : Z) :
+    pure (eval η e1) (λ x1', x1' = x1) ⊥ ->
+    pure (eval η e2) (λ x2', x2' = x2) ⊥ ->
+    (* Representability hypotheses last for [x1] and [x2] evar initialisation *)
+    representable x1 ->
+    representable x2 ->
+    pure (eval η (EOpEq e1 e2)) (λ P, P <-> (x1 = x2)%Z) ⊥.
+  Proof.
+    intros He1 He2 Hx1 Hx2. simpl_eval.
+    eapply pure_eval_comparison_operator; eauto.
+    rewrite eq_repr_repr; auto.
+    simpl. f_equal. f_equal. apply truth_eq_true. lia.
+  Qed.
 
-  (* Lemma pure_eval_EOpGt_bool η e1 e2 (x1 x2 : Z) : *)
-  (*   pure (eval η e1) ##(λ x1', x1' = x1) ⊥ -> *)
-  (*   pure (eval η e2) ##(λ x2', x2' = x2) ⊥ -> *)
-  (*   (* Representability hypotheses last for [x1] and [x2] evar initialisation *) *)
-  (*   representable x1 -> *)
-  (*   representable x2 -> *)
-  (*   pure (eval η (EOpGt e1 e2)) ##(λ (b : bool), b <-> (x1 > x2)) ⊥. *)
-  (* Proof. *)
-  (*   intros. eapply pure_mono_ret. eapply pure_eval_EOpGt; eauto. *)
-  (*   intros _ (P & -> & HP). exists (truth P). by rewrite <-HP, encode_truth, Is_true_truth. *)
-  (* Qed. *)
+  Lemma pure_eval_EOpEq_bool η e1 e2 (x1 x2 : Z) :
+    pure (eval η e1) (λ x1', x1' = x1) ⊥ ->
+    pure (eval η e2) (λ x2', x2' = x2) ⊥ ->
+    (* Representability hypotheses last for [x1] and [x2] evar initialisation *)
+    representable x1 ->
+    representable x2 ->
+    pure (eval η (EOpEq e1 e2)) (λ (b : bool), b <-> (x1 = x2)) ⊥.
+  Proof.
+    intros. eapply pure_wp_mono_ret. eapply pure_eval_EOpEq; eauto.
+    intros _ (P & -> & HP). exists (truth P). by rewrite <-HP, encode_truth, Is_true_truth.
+  Qed.
 
-  (* Lemma pure_eval_EOpGe η e1 e2 (x1 x2 : Z) : *)
-  (*   pure (eval η e1) ##(λ x1', x1' = x1) ⊥ -> *)
-  (*   pure (eval η e2) ##(λ x2', x2' = x2) ⊥ -> *)
-  (*   (* Representability hypotheses last for [x1] and [x2] evar initialisation *) *)
-  (*   representable x1 -> *)
-  (*   representable x2 -> *)
-  (*   pure (eval η (EOpGe e1 e2)) ##(λ P, P <-> (x1 >= x2)%Z) ⊥. *)
-  (* Proof. *)
-  (*   intros He1 He2 Hx1 Hx2. simpl_eval. *)
-  (*   eapply pure_eval_comparison_operator; eauto. *)
-  (*   rewrite lt_repr_repr; auto. *)
-  (*   simpl. f_equal. f_equal. apply truth_eq_true. lia. *)
-  (* Qed. *)
+  Lemma pure_eval_EOpNe η e1 e2 (x1 x2 : Z) :
+    pure (eval η e1) (λ x1', x1' = x1) ⊥ ->
+    pure (eval η e2) (λ x2', x2' = x2) ⊥ ->
+    (* Representability hypotheses last for [x1] and [x2] evar initialisation *)
+    representable x1 ->
+    representable x2 ->
+    pure (eval η (EOpNe e1 e2)) (λ P, P <-> (x1 <> x2)%Z) ⊥.
+  Proof.
+    intros He1 He2 Hx1 Hx2. simpl_eval.
+    eapply pure_eval_comparison_operator; eauto.
+    rewrite eq_repr_repr; auto.
+    simpl. f_equal. f_equal. apply truth_eq_true. lia.
+  Qed.
 
-  (* Lemma pure_eval_EOpGe_bool η e1 e2 (x1 x2 : Z) : *)
-  (*   pure (eval η e1) ##(λ x1', x1' = x1) ⊥ -> *)
-  (*   pure (eval η e2) ##(λ x2', x2' = x2) ⊥ -> *)
-  (*   (* Representability hypotheses last for [x1] and [x2] evar initialisation *) *)
-  (*   representable x1 -> *)
-  (*   representable x2 -> *)
-  (*   pure (eval η (EOpGe e1 e2)) ##(λ (b : bool), b <-> (x1 >= x2)) ⊥. *)
-  (* Proof. *)
-  (*   intros. eapply pure_mono_ret. eapply pure_eval_EOpGe; eauto. *)
-  (*   intros _ (P & -> & HP). exists (truth P). by rewrite <-HP, encode_truth, Is_true_truth. *)
-  (* Qed. *)
+  Lemma pure_eval_EOpNe_bool η e1 e2 (x1 x2 : Z) :
+    pure (eval η e1) (λ x1', x1' = x1) ⊥ ->
+    pure (eval η e2) (λ x2', x2' = x2) ⊥ ->
+    (* Representability hypotheses last for [x1] and [x2] evar initialisation *)
+    representable x1 ->
+    representable x2 ->
+    pure (eval η (EOpNe e1 e2)) (λ (b : bool), b <-> (x1 <> x2)) ⊥.
+  Proof.
+    intros. eapply pure_wp_mono_ret. eapply pure_eval_EOpNe; eauto.
+    intros _ (P & -> & HP). exists (truth P). by rewrite <-HP, encode_truth, Is_true_truth.
+  Qed.
 
-  (* Lemma pure_eval_EOpEq η e1 e2 (x1 x2 : Z) : *)
-  (*   pure (eval η e1) ##(λ x1', x1' = x1) ⊥ -> *)
-  (*   pure (eval η e2) ##(λ x2', x2' = x2) ⊥ -> *)
-  (*   (* Representability hypotheses last for [x1] and [x2] evar initialisation *) *)
-  (*   representable x1 -> *)
-  (*   representable x2 -> *)
-  (*   pure (eval η (EOpEq e1 e2)) ##(λ P, P <-> (x1 = x2)%Z) ⊥. *)
-  (* Proof. *)
-  (*   intros He1 He2 Hx1 Hx2. simpl_eval. *)
-  (*   eapply pure_eval_comparison_operator; eauto. *)
-  (*   rewrite eq_repr_repr; auto. *)
-  (*   simpl. f_equal. f_equal. apply truth_eq_true. lia. *)
-  (* Qed. *)
+  (* Runtime assertions. *)
 
-  (* Lemma pure_eval_EOpEq_bool η e1 e2 (x1 x2 : Z) : *)
-  (*   pure (eval η e1) ##(λ x1', x1' = x1) ⊥ -> *)
-  (*   pure (eval η e2) ##(λ x2', x2' = x2) ⊥ -> *)
-  (*   (* Representability hypotheses last for [x1] and [x2] evar initialisation *) *)
-  (*   representable x1 -> *)
-  (*   representable x2 -> *)
-  (*   pure (eval η (EOpEq e1 e2)) ##(λ (b : bool), b <-> (x1 = x2)) ⊥. *)
-  (* Proof. *)
-  (*   intros. eapply pure_mono_ret. eapply pure_eval_EOpEq; eauto. *)
-  (*   intros _ (P & -> & HP). exists (truth P). by rewrite <-HP, encode_truth, Is_true_truth. *)
-  (* Qed. *)
+  Lemma pure_eval_assert_bool η e :
+    pure (eval η e) (λ b, b = true) ⊥ →
+    pure (eval η (EAssert e)) (λ (_ : unit), True) ⊥.
+  Proof.
+    intros He.
+    eapply pure_wp_mono_ret.
+    eapply pure_assert.
+    eapply pure_wp_mono_ret.
+    eapply He.
+    all:intros _ (V & -> & ->); repeat econstructor.
+  Qed.
 
-  (* Lemma pure_eval_EOpNe η e1 e2 (x1 x2 : Z) : *)
-  (*   pure (eval η e1) ##(λ x1', x1' = x1) ⊥ -> *)
-  (*   pure (eval η e2) ##(λ x2', x2' = x2) ⊥ -> *)
-  (*   (* Representability hypotheses last for [x1] and [x2] evar initialisation *) *)
-  (*   representable x1 -> *)
-  (*   representable x2 -> *)
-  (*   pure (eval η (EOpNe e1 e2)) ##(λ P, P <-> (x1 <> x2)%Z) ⊥. *)
-  (* Proof. *)
-  (*   intros He1 He2 Hx1 Hx2. simpl_eval. *)
-  (*   eapply pure_eval_comparison_operator; eauto. *)
-  (*   rewrite eq_repr_repr; auto. *)
-  (*   simpl. f_equal. f_equal. apply truth_eq_true. lia. *)
-  (* Qed. *)
+  Lemma pure_eval_assert_Prop η e :
+    pure (eval η e) (λ P : Prop, P) ⊥ →
+    pure (eval η (EAssert e)) (λ (_ : unit), True) ⊥.
+  Proof.
+    intros He.
+    eapply pure_wp_mono_ret.
+    eapply pure_assert.
+    eapply pure_wp_mono_ret.
+    eapply He.
+    - intros _ (P & -> & HP).
+      unfold encode, Encode_bool, Encode_Prop. rewrite truth_true; eauto.
+      repeat econstructor.
+    - intros _ (V & -> & ->); repeat econstructor.
+  Qed.
 
-  (* Lemma pure_eval_EOpNe_bool η e1 e2 (x1 x2 : Z) : *)
-  (*   pure (eval η e1) ##(λ x1', x1' = x1) ⊥ -> *)
-  (*   pure (eval η e2) ##(λ x2', x2' = x2) ⊥ -> *)
-  (*   (* Representability hypotheses last for [x1] and [x2] evar initialisation *) *)
-  (*   representable x1 -> *)
-  (*   representable x2 -> *)
-  (*   pure (eval η (EOpNe e1 e2)) ##(λ (b : bool), b <-> (x1 <> x2)) ⊥. *)
-  (* Proof. *)
-  (*   intros. eapply pure_mono_ret. eapply pure_eval_EOpNe; eauto. *)
-  (*   intros _ (P & -> & HP). exists (truth P). by rewrite <-HP, encode_truth, Is_true_truth. *)
-  (* Qed. *)
+  (* Sequencing of pure computations. *)
 
-  (* (* Runtime assertions. *) *)
+  Lemma pure_seq φ ψ η e1 e2 :
+    pure (eval η e1) (λ _, pure (eval η e2) φ ψ) ψ →
+    pure (eval η (ESeq e1 e2)) φ ψ.
+  Proof.
+    simpl_eval.
+    intros. apply pure_wp_bind.
+    eapply pure_wp_mono; try done.
+    intros; eapply pure_wp_mono; first eapply H0; try done.
+    intros ? (?&?&?); subst; try done.
+  Qed.
 
-  (* Lemma pure_eval_assert_bool η e : *)
-  (*   pure (eval η e) ##(λ b, b = true) ⊥ → *)
-  (*   pure (eval η (EAssert e)) ##(λ (_ : unit), True) ⊥. *)
-  (* Proof. *)
-  (*   intros He. *)
-  (*   eapply pure_mono_ret. *)
-  (*   eapply pure_assert. *)
-  (*   eapply pure_mono_ret. *)
-  (*   eapply He. *)
-  (*   - by intros _ (V & -> & ->). *)
-  (*   - intros _ ->. eauto with encode. *)
-  (* Qed. *)
+  Lemma pure_eval_seq' `{Encode A}
+    η e1 e2 (ψ : A -> Prop) :
+    pure (eval η e1) (λ _, True) ⊥ ->
+    pure (eval η e2) ψ ⊥ ->
+    pure (eval η (ESeq e1 e2)) ψ ⊥.
+  Proof.
+    intros He1 He2.
+    apply pure_seq.
+    apply (pure_wp_mono_ret _ He1). intros _ _.
+    apply (pure_wp_mono_ret _ He2).
+    apply returns_idem.
+  Qed.
 
-  (* Lemma pure_eval_assert_Prop η e : *)
-  (*   pure (eval η e) ##(λ P : Prop, P) ⊥ → *)
-  (*   pure (eval η (EAssert e)) ##(λ (_ : unit), True) ⊥. *)
-  (* Proof. *)
-  (*   intros He. *)
-  (*   eapply pure_mono_ret. *)
-  (*   eapply pure_assert. *)
-  (*   eapply pure_mono_ret. *)
-  (*   eapply He. *)
-  (*   - intros _ (P & -> & HP). *)
-  (*     unfold encode, Encode_bool, Encode_Prop. by rewrite truth_true. *)
-  (*   - intros _ ->. eauto with encode. *)
-  (* Qed. *)
+  Lemma pure_eval_seq `{Encode A, Encode B}
+    η e1 e2 (ψ : A -> Prop) :
+    pure (eval η e1) (λ _ : B, True) ⊥ ->
+    pure (eval η e2) ψ ⊥ ->
+    pure (eval η (ESeq e1 e2)) ψ ⊥.
+  Proof.
+    intros He1 He2.
+    apply pure_seq.
+    apply (pure_wp_mono_ret _ He1). intros _ _.
+    apply (pure_wp_mono_ret _ He2).
+    apply returns_idem.
+  Qed.
 
-  (* (* Sequencing of pure computations. *) *)
+  Lemma pure_eval_seq_exn `{Encode A}
+    η e1 e2 (Ψ : A -> Prop) ζ :
+    pure (eval η e1) (λ _ : val, pure (eval η e2) Ψ ζ) ζ ->
+    pure (eval η (ESeq e1 e2)) Ψ ζ.
+  Proof.
+    intros Hpure. apply pure_seq.
+    eapply (pure_wp_mono _ Hpure); last auto.
+    intros ? (? & -> & ?).
+    eapply (pure_wp_mono _ H0); last auto.
+    apply returns_idem.
+  Qed.
 
-  (* Lemma pure_eval_seq' `{Encode A} η e1 e2 (ψ : A -> Prop) : *)
-  (*   pure (eval η e1) (λ _, True) ⊥ -> *)
-  (*   pure (eval η e2) ##ψ ⊥ -> *)
-  (*   pure (eval η (ESeq e1 e2)) ##ψ ⊥. *)
-  (* Proof. *)
-  (*   intros He1 He2. *)
-  (*   apply pure_seq. *)
-  (*   apply (pure_mono_ret _ He1). intros _ _. *)
-  (*   apply (pure_mono_ret _ He2). intuition. *)
-  (* Qed. *)
-
-  (* Lemma pure_eval_seq `{Encode A} `{Encode B} η e1 e2 (ψ : A -> Prop) : *)
-  (*   pure (eval η e1) ##(λ _ : B, True) ⊥ -> *)
-  (*   pure (eval η e2) ##ψ ⊥ -> *)
-  (*   pure (eval η (ESeq e1 e2)) ##ψ ⊥. *)
-  (* Proof. *)
-  (*   intros He1 He2. *)
-  (*   apply pure_seq. *)
-  (*   apply (pure_mono_ret _ He1). intros _ _. *)
-  (*   apply (pure_mono_ret _ He2). intuition. *)
-  (* Qed. *)
-
-  (* Lemma pure_eval_seq_exn `{Encode A} η e1 e2 (Ψ : A -> Prop) ζ : *)
-  (*   pure (eval η e1) ##(λ _ : val, pure (eval η e2) ##Ψ ζ) ζ -> *)
-  (*   pure (eval η (ESeq e1 e2)) ##Ψ ζ. *)
-  (* Proof. *)
-  (*   intros Hpure. apply pure_seq. *)
-  (*   eapply (pure_mono _ Hpure); last auto. *)
-  (*   by intros ? (? & ? & ?). *)
-  (* Qed. *)
-
-  (* Lemma pure_eval_mexpr_struct (η δ whatenv : env) items (ψ : val -> Prop) : *)
-  (*   simp (eval_sitems (η, []) items) (ret (whatenv, δ)) -> *)
-  (*   ψ (VStruct δ) -> *)
-  (*   pure (eval_mexpr η (MStruct items)) ##ψ ⊥. *)
-  (* Proof. *)
-  (*   intros. simpl_eval_mexpr. *)
-  (*   eapply pure_simp; [ simp | eauto using pure_ret with encode ]. *)
-  (* Qed. *)
+  Lemma pure_eval_mexpr_struct (η δ whatenv : env) items (ψ : val -> Prop) :
+    simp (eval_sitems (η, []) items) (ret (whatenv, δ)) ->
+    ψ (VStruct δ) ->
+    pure (eval_mexpr η (MStruct items)) ψ ⊥.
+  Proof.
+    intros. simpl_eval_mexpr.
+    eapply pure_wp_simp; [ simp | eauto using pure_wp_ret with pure ].
+  Qed.
 
   (* Lemma pure_eval_mexpr_coerc η me c v (ψ : val -> Prop): *)
   (*   simp (eval_mexpr η me) (ret v) -> *)
-  (*   pure (coerce c v) ##ψ ⊥ -> *)
-  (*   pure (eval_mexpr η (MCoercion me c)) ##ψ ⊥. *)
+  (*   pure (coerce c v) ψ ⊥ -> *)
+  (*   pure (eval_mexpr η (MCoercion me c)) ψ ⊥. *)
   (* Proof. *)
   (*   intros Hme Hc. simpl_eval_mexpr. eapply pure_bind. *)
-  (*   eapply pure_simp; eauto. *)
-  (*   eapply pure_mono_ret. eapply pure_ret_eq. *)
-  (*   intros _ ->. *)
-  (*   rewrite pure_widen'. *)
+  (*   eapply pure_wp_simp; eauto. *)
+  (*   eapply pure_wp_mono_ret. eapply pure_wp_ret_eq. *)
+  (*   intros _ ->. eauto with pure *)
+  (*   rewrite pure_wp_widen'. *)
   (*   apply Hc. *)
   (* Qed. *)
 
-  (* Lemma pure_eval_ret_concat `{Encode A} e δ η (ψ : A -> Prop) ζ : *)
-  (*   pure (eval (δ ++ η) e) ##ψ ζ -> *)
-  (*   pure (θ ← ret (δ ++ η); *)
-  (*         eval θ e) ##ψ ζ. *)
-  (* Proof. *)
-  (*   tauto. *)
-  (* Qed. *)
+  Lemma pure_eval_ret_concat `{Encode A}
+    e δ η (ψ : A -> Prop) ζ :
+    pure (eval (δ ++ η) e) ψ ζ ->
+    pure (θ ← ret (δ ++ η);
+          eval θ e) ψ ζ.
+  Proof.
+    tauto.
+  Qed.
 
-  (* Lemma pure_eval_const `{Encode X} η c x (ψ : X -> Prop) ζ : *)
-  (*   VConstant c = #x -> *)
-  (*   ψ x -> *)
-  (*   pure (eval η (EConstant c)) ψ ζ. *)
-  (* Proof. *)
-  (*   intros. *)
-  (*   eapply pure_simp. simp. *)
-  (*   eauto using pure_ret with pure. *)
-  (* Qed. *)
-
-  (* Lemma pure_eval_data `{Encode Y} η c e y (ψ : Y -> Prop) ζ : *)
-  (*   pure (eval η e) (λ v', VData c v' = #y) ζ -> *)
-  (*   ψ y -> *)
-  (*   pure (eval η (EData c e)) ψ ζ. *)
-  (* Proof. *)
-  (*   intros He Hy. *)
-  (*   simpl_eval. *)
-  (*   eapply pure_bind. *)
-  (* (*   eapply pure_consequence; eauto. *) *)
-  (* (*   intros ? A. *) *)
-  (* (*   eapply pure_noexn_weaken, pure_enc_ret; eauto; auto. *) *)
-  (* (* Qed. *) *)
-  (* Admitted. *)
-
+  Lemma pure_eval_const `{Encode A}
+    η c x (ψ : A -> Prop) ζ :
+    VConstant c = #x ->
+    ψ x ->
+    pure (eval η (EConstant c)) ψ ζ.
+  Proof.
+    intros.
+    eapply pure_wp_simp. simp.
+    eauto using pure_ret with pure.
+  Qed.
 
 End eval_rules.
 
-(* TODO Clean up and comment *)
-Ltac pure_eval_path :=
-  eexists _, _;
-  eapply pure_eval_path, total_ret_eq_and.
-Ltac pure_data :=
-  eapply pure_eval_data;
-  first try done;
-  repeat pure_eval_path; exists eq_refl.
-Ltac pure_match :=
-  eapply pure_match_cons; first solve_pattern; last intuition.
-Ltac pure_path := by eapply pure_eval_path, total_ret.
-Ltac eval_match :=
-  eapply pure_eval_match; first pure_path.
-Ltac match_signature hd :=
-  eapply (@pure_evals_cons hd);
-  eapply pure_eval_path; cbn -[evals];
-  apply pure_wp_ret; eexists _; split; first done.
-Ltac match_signatures l :=
-  match l with
-  | cons ?hd ?tl => match_signature hd;
-                    match_signatures tl
-  | nil => simpl_evals; apply pure_wp_ret; auto
-  end.
-Tactic Notation "build" "(" constr(x) ":" constr(l) ")":=
-  apply (pure_eval_data_eq x); first match_signatures l.
+Lemma pure_eval_data `{Encode Y} η c e y (ψ : Y -> Prop) ζ :
+  pure (evals η e) (λ v', VData c v' = #y) ζ ->
+  ψ y ->
+  pure (eval η (EData c e)) ψ ζ.
+Proof.
+  intros He Hy.
+  simpl_eval.
+  eapply pure_wp_bind.
+  eapply pure_wp_mono; eauto.
+  intros ? ?; eapply pure_wp_noexn_weaken. eauto with pure.
+Qed.
+
+
+
