coq-osiris/theories/program_logic/pure/pattern_rules.v
@@ -18,113 +18,113 @@ Open Scope Z_scope.
    results in an extended environment that satisfies [φ]
    or fails (by reducing to [throw ()]) and guarantees [ψ]. *)
 
-Definition cpattern_wp η p o (φ : env -> Prop) (ψ : Prop) :=
+Definition cpattern η p o (φ : env -> Prop) (ψ : Prop) :=
   pure_wp (cextend η p o) φ (λ (_ : unit), ψ).
 
-Definition pattern_wp η p v (φ : env -> Prop) (ψ : Prop) :=
+Definition pattern η p v (φ : env -> Prop) (ψ : Prop) :=
   pure_wp (extend η p v) φ (λ (_ : unit), ψ).
 
-Definition patterns_wp η ps vs (φ : env -> Prop) (ψ : Prop) :=
+Definition patterns η ps vs (φ : env -> Prop) (ψ : Prop) :=
   pure_wp (extends η ps vs) φ (λ (_ : unit), ψ).
 
 (* -------------------------------------------------------------------------- *)
 
-(* cpattern_wp : env → cpat → outcome.outcome3 val locations.loc val val → (env → Prop) → Prop → Prop *)
-(* pattern_wp : env → pat → val → (env → Prop) → Prop → Prop *)
-(* patterns_wp : env → list pat → list val → (env → Prop) → Prop → Prop *)
+(* cpattern : env → cpat → outcome.outcome3 val locations.loc val val → (env → Prop) → Prop → Prop *)
+(* pattern : env → pat → val → (env → Prop) → Prop → Prop *)
+(* patterns : env → list pat → list val → (env → Prop) → Prop → Prop *)
 
-(* Class pattern_wp_template := *)
-(*   { pattern_wp_shape : Type; pattern_wp_outcome : Type }. *)
+(* Class pattern_template := *)
+(*   { pattern_shape : Type; pattern_outcome : Type }. *)
 
-(* Class pat {P : pattern_wp_template} := *)
-(*   pat_ : env -> pattern_wp_shape -> pattern_wp_outcome -> (env -> Prop) -> Prop -> Prop. *)
+(* Class pat {P : pattern_template} := *)
+(*   pat_ : env -> pattern_shape -> pattern_outcome -> (env -> Prop) -> Prop -> Prop. *)
 
 (* -------------------------------------------------------------------------- *)
 
-Section pattern_wp_rules.
+Section pattern_rules.
 
   Implicit Type φ : env -> Prop.
   Implicit Type ψ : Prop.
 
-  (* Monotonicity properties for [cpattern_wp], [pattern_wp], and [patterns_wp]. *)
+  (* Monotonicity properties for [cpattern], [pattern], and [patterns]. *)
 
-  Lemma cpattern_wp_mono η p v (φ φ' : env -> Prop) (ψ ψ' : Prop) :
-    cpattern_wp η p v φ ψ →
+  Lemma cpattern_mono η p v (φ φ' : env -> Prop) (ψ ψ' : Prop) :
+    cpattern η p v φ ψ →
     (∀ η, φ η → φ' η) →
     (ψ → ψ') →
-    cpattern_wp η p v φ' ψ'.
+    cpattern η p v φ' ψ'.
   Proof.
-    unfold cpattern_wp; eauto using pure_wp_mono.
+    unfold cpattern; eauto using pure_wp_mono.
   Qed.
 
-  Lemma cpattern_wp_env_mono η p v (φ φ' : env -> Prop) (ψ : Prop) :
-    cpattern_wp η p v φ ψ →
+  Lemma cpattern_env_mono η p v (φ φ' : env -> Prop) (ψ : Prop) :
+    cpattern η p v φ ψ →
     (∀ η, φ η → φ' η) →
-    cpattern_wp η p v φ' ψ.
-  Proof. intros; by eapply cpattern_wp_mono. Qed.
+    cpattern η p v φ' ψ.
+  Proof. intros; by eapply cpattern_mono. Qed.
 
-  Lemma cpattern_wp_exn_mono η p v (φ : env -> Prop) (ψ ψ': Prop) :
-    cpattern_wp η p v φ ψ →
+  Lemma cpattern_exn_mono η p v (φ : env -> Prop) (ψ ψ': Prop) :
+    cpattern η p v φ ψ →
     (ψ → ψ') →
-    cpattern_wp η p v φ ψ'.
-  Proof. intros; by eapply cpattern_wp_mono. Qed.
+    cpattern η p v φ ψ'.
+  Proof. intros; by eapply cpattern_mono. Qed.
 
-  Lemma pattern_wp_mono η p v (φ φ' : env -> Prop) (ψ ψ' : Prop) :
-    pattern_wp η p v φ ψ →
+  Lemma pattern_mono η p v (φ φ' : env -> Prop) (ψ ψ' : Prop) :
+    pattern η p v φ ψ →
     (∀ η, φ η → φ' η) →
     (ψ → ψ') →
-    pattern_wp η p v φ' ψ'.
+    pattern η p v φ' ψ'.
   Proof.
-    unfold pattern_wp; eauto using pure_wp_mono.
+    unfold pattern; eauto using pure_wp_mono.
   Qed.
 
-  Lemma pattern_wp_env_mono η p v (φ φ' : env -> Prop) (ψ : Prop) :
-    pattern_wp η p v φ ψ →
+  Lemma pattern_env_mono η p v (φ φ' : env -> Prop) (ψ : Prop) :
+    pattern η p v φ ψ →
     (∀ η, φ η → φ' η) →
-    pattern_wp η p v φ' ψ.
-  Proof. intros; by eapply pattern_wp_mono. Qed.
+    pattern η p v φ' ψ.
+  Proof. intros; by eapply pattern_mono. Qed.
 
-  Lemma pattern_wp_exn_mono η p v (φ : env -> Prop) (ψ ψ': Prop) :
-    pattern_wp η p v φ ψ →
+  Lemma pattern_exn_mono η p v (φ : env -> Prop) (ψ ψ': Prop) :
+    pattern η p v φ ψ →
     (ψ → ψ') →
-    pattern_wp η p v φ ψ'.
-  Proof. intros; by eapply pattern_wp_mono. Qed.
+    pattern η p v φ ψ'.
+  Proof. intros; by eapply pattern_mono. Qed.
 
-  Lemma patterns_wp_mono η p v (φ φ' : env -> Prop) (ψ ψ' : Prop) :
-    patterns_wp η p v φ ψ →
+  Lemma patterns_mono η p v (φ φ' : env -> Prop) (ψ ψ' : Prop) :
+    patterns η p v φ ψ →
     (∀ η, φ η → φ' η) →
     (ψ → ψ') →
-    patterns_wp η p v φ' ψ'.
+    patterns η p v φ' ψ'.
   Proof.
-    unfold patterns_wp; eauto using pure_wp_mono.
+    unfold patterns; eauto using pure_wp_mono.
   Qed.
 
-  Lemma patterns_wp_env_mono η p v (φ φ' : env -> Prop) (ψ : Prop) :
-    patterns_wp η p v φ ψ →
+  Lemma patterns_env_mono η p v (φ φ' : env -> Prop) (ψ : Prop) :
+    patterns η p v φ ψ →
     (∀ η, φ η → φ' η) →
-    patterns_wp η p v φ' ψ.
-  Proof. intros; by eapply patterns_wp_mono. Qed.
+    patterns η p v φ' ψ.
+  Proof. intros; by eapply patterns_mono. Qed.
 
-  Lemma patterns_wp_exn_mono η p v (φ : env -> Prop) (ψ ψ': Prop) :
-    patterns_wp η p v φ ψ →
+  Lemma patterns_exn_mono η p v (φ : env -> Prop) (ψ ψ': Prop) :
+    patterns η p v φ ψ →
     (ψ → ψ') →
-    patterns_wp η p v φ ψ'.
-  Proof. intros; by eapply patterns_wp_mono. Qed.
+    patterns η p v φ ψ'.
+  Proof. intros; by eapply patterns_mono. Qed.
 
   (* -------------------------------------------------------------------------- *)
 
-  (* Syntax-directed reasoning rules for the judgement [pattern_wp]. *)
+  (* Syntax-directed reasoning rules for the judgement [pattern]. *)
 
   (* From an operational point of view, the repeated application of these
-    lemmas to a pattern_wp [p] and a value [v] have the effect of translating
-    the pattern_wp matching operation [p = v] into a positive formula and a
+    lemmas to a pattern [p] and a value [v] have the effect of translating
+    the pattern matching operation [p = v] into a positive formula and a
     negative formula. The positive formula, the postcondition [φ],
     accumulates a sequence of universal quantifiers and equations that
-    describe what is learnt when pattern_wp matching succeeds. The negative
+    describe what is learnt when pattern matching succeeds. The negative
     formula, the failure postcondition [ψ], describes what is learnt when
-    pattern_wp matching fails. *)
+    pattern matching fails. *)
 
-  (* When a pattern_wp cannot fail or can fail due to several distinct causes,
+  (* When a pattern cannot fail or can fail due to several distinct causes,
     a naive statement of its reasoning rule would have one occurrence of
     [ψ] in its conclusion and no occurrence or multiple occurrences of [ψ]
     in its premises. From an operational point of view, this is
@@ -136,88 +136,88 @@ Section pattern_wp_rules.
 
   Lemma pat_PAny η v φ :
     φ η →
-    pattern_wp η PAny v φ False.
+    pattern η PAny v φ False.
   Proof.
-    unfold pattern_wp. simpl_extend. eauto using pure_wp_ret.
+    unfold pattern. simpl_extend. eauto using pure_wp_ret.
   Qed.
 
   Lemma pat_PVar η x v φ :
     φ ((x, v) :: η) →
-    pattern_wp η (PVar x) v φ False.
+    pattern η (PVar x) v φ False.
   Proof.
-    unfold pattern_wp. simpl_extend. eauto using pure_wp_ret.
+    unfold pattern. simpl_extend. eauto using pure_wp_ret.
   Qed.
 
-  (* Given a goal of the form [pattern_wp η (PVar x) v ?φ False],
+  (* Given a goal of the form [pattern η (PVar x) v ?φ False],
     applying the lemma [pat_PVar2] solves the goal and
     instantiates the postcondition [?φ]. *)
 
   Lemma pat_PVar2 η x v :
-    pattern_wp η (PVar x) v (λ η', η' = (x, v) :: η) False.
+    pattern η (PVar x) v (λ η', η' = (x, v) :: η) False.
   Proof.
     by apply pat_PVar.
   Qed.
 
   Ltac pat_PVar :=
     match goal with
-    | |- pattern_wp _ (PVar _) _ _ _ =>
+    | |- pattern _ (PVar _) _ _ _ =>
         (apply pat_PVar2 || eapply pat_PVar)
     end.
 
   Lemma pat_PAlias η p x v φ ψ :
-    pattern_wp η p v (λ η, φ ((x, v) :: η)) ψ →
-    pattern_wp η (PAlias p x) v φ ψ.
+    pattern η p v (λ η, φ ((x, v) :: η)) ψ →
+    pattern η (PAlias p x) v φ ψ.
   Proof.
-    unfold pattern_wp. simpl_extend; intros.
+    unfold pattern. simpl_extend; intros.
     apply pure_wp_bind.
     eauto using pure_wp_mono, pure_wp_ret.
   Qed.
 
-  (* TODO generalize to [(φ1 η → pattern_wp η p2 v φ ψ2)] and see if it is useful *)
+  (* TODO generalize to [(φ1 η → pattern η p2 v φ ψ2)] and see if it is useful *)
   Lemma pat_POr η p1 p2 v φ ψ1 ψ2 :
-    pattern_wp η p1 v φ ψ1 →
-    pattern_wp η p2 v φ ψ2 →
-    pattern_wp η (POr p1 p2) v φ (ψ1 ∧ ψ2).
+    pattern η p1 v φ ψ1 →
+    pattern η p2 v φ ψ2 →
+    pattern η (POr p1 p2) v φ (ψ1 ∧ ψ2).
       (* The conjunction [ψ1 ∧ ψ2] reflects the fact that, for the
-        disjunction pattern_wp to fail, both sides must fail. *)
+        disjunction pattern to fail, both sides must fail. *)
   Proof.
-    unfold pattern_wp. simpl_extend; intros.
+    unfold pattern. simpl_extend; intros.
     eauto using pure_wp_orelse, pure_wp_mono.
   Qed.
 
   Lemma pat_PUnit η v φ :
     φ η →
     v = #() →
-    pattern_wp η PUnit v φ False.
+    pattern η PUnit v φ False.
   Proof.
-    unfold pattern_wp. intros ? ->; simpl_extend.
+    unfold pattern. intros ? ->; simpl_extend.
     eauto using pure_wp_ret.
   Qed.
 
   Lemma pat_PTuple `{Encode A} η ps (a : A) vs φ ψ :
     #a = VTuple vs ->
-    patterns_wp η ps vs φ ψ →
-    pattern_wp η (PTuple ps) #a φ ψ.
+    patterns η ps vs φ ψ →
+    pattern η (PTuple ps) #a φ ψ.
   Proof.
-    unfold patterns_wp, pattern_wp.
+    unfold patterns, pattern.
     intros ->. by simpl_extend.
   Qed.
 
   Lemma pat_PTuple_val η ps vs φ ψ :
-    patterns_wp η ps vs φ ψ ->
-    pattern_wp η (PTuple ps) (VTuple vs) φ ψ.
+    patterns η ps vs φ ψ ->
+    pattern η (PTuple ps) (VTuple vs) φ ψ.
   Proof.
-    unfold pattern_wp. by simpl_extend.
+    unfold pattern. by simpl_extend.
   Qed.
 
   Lemma pat_PPair `{Encode A, Encode B} η p1 p2 v1 v2 (x1 : A) (x2 : B) φ ψ1 ψ2 :
     v1 = #x1 ->
     v2 = #x2 ->
-    pattern_wp η p1 #x1 (λ η', pattern_wp η' p2 #x2 φ (ψ2)) (ψ1) ->
-    pattern_wp η (PPair p1 p2) (VPair v1 v2) φ (ψ1 \/ ψ2).
+    pattern η p1 #x1 (λ η', pattern η' p2 #x2 φ (ψ2)) (ψ1) ->
+    pattern η (PPair p1 p2) (VPair v1 v2) φ (ψ1 \/ ψ2).
   Proof.
     intros; subst.
-    unfold pattern_wp. simpl_extend.
+    unfold pattern. simpl_extend.
     eapply pure_wp_bind_conseq; [ eapply pure_wp_mono; eauto | ].
     simpl; intros. rewrite bind_ret_right.
     eapply pure_wp_bind_conseq; [ eapply pure_wp_mono; eauto | ].
@@ -226,52 +226,61 @@ Section pattern_wp_rules.
 
   Lemma pat_PData_nil η c c' φ ψ :
     (c = c' -> φ η) ->
-    pattern_wp η (PData c nil) (VData c' nil) φ (ψ ∨ c ≠ c').
+    pattern η (PData c nil) (VData c' nil) φ (ψ ∨ c ≠ c').
       (* This form is useful when the truth of the equality [c = c']
         is not statically known. *)
   Proof.
-    unfold pattern_wp; intros. simpl_extend.
+    unfold pattern; intros. simpl_extend.
     destruct_string_eqb;
-      eauto using pure_wp_throw, pure_wp_mono, pure_wp_ret.
+      eauto using pure_wp_throw, pure_mono, pure_wp_ret.
   Qed.
 
-  Lemma pat_PData η c c' p v φ ψ :
-    (c = c' -> patterns_wp η p v φ ψ) ->
-    pattern_wp η (PData c p) (VData c' v) φ (ψ ∨ c ≠ c').
+  Lemma pat_PData_or η c c' p v φ ψ :
+    (c = c' -> patterns η p v φ ψ) ->
+    pattern η (PData c p) (VData c' v) φ (ψ ∨ c ≠ c').
       (* This form is useful when the truth of the equality [c = c']
         is not statically known. *)
   Proof.
-    unfold pattern_wp; intros. simpl_extend.
+    unfold pattern; intros. simpl_extend.
     destruct_string_eqb; eauto using pure_wp_throw.
     eapply pure_wp_mono; first apply H; eauto.
   Qed.
 
   Lemma pat_PData_eq η c p v φ ψ :
-    patterns_wp η p v φ ψ →
-    pattern_wp η (PData c p) (VData c v) φ ψ.
+    patterns η p v φ ψ →
+    pattern η (PData c p) (VData c v) φ ψ.
       (* This form is useful when [c = c'] is statically known. *)
   Proof.
-    unfold pattern_wp; intros. simpl_extend.
+    unfold pattern; intros. simpl_extend.
     destruct_string_eqb; solve [ eauto using pure_wp_throw | tauto ].
   Qed.
 
   Lemma pat_PData_neq η c p c' v φ :
     c ≠ c' →
-    pattern_wp η (PData c p) (VData c' v) φ True.
+    pattern η (PData c p) (VData c' v) φ True.
       (* This form is useful when [c ≠ c'] is statically known. *)
   Proof.
-    unfold pattern_wp; intros. simpl_extend.
+    unfold pattern; intros. simpl_extend.
+    destruct_string_eqb; solve [ eauto using pure_wp_throw | tauto ].
+  Qed.
+
+  Lemma pat_PData η c p c' v v' φ :
+    v = VData c' v' ->
+    (c = c' -> patterns η p v' φ True) ->
+    pattern η (PData c p) v φ True.
+  Proof.
+    unfold pattern; intros. simpl_extend. subst.
     destruct_string_eqb; solve [ eauto using pure_wp_throw | tauto ].
   Qed.
 
   Lemma pat_PXData_eq η c p c' v φ ψ :
     lookup_path η c = ret (VLoc c') ->
-    patterns_wp η p v φ ψ →
-    pattern_wp η (PXData c p) (VXData c' v) φ ψ.
+    patterns η p v φ ψ →
+    pattern η (PXData c p) (VXData c' v) φ ψ.
       (* This form is useful when the truth of the equality [c = c']
         is not statically known. *)
   Proof.
-    unfold pattern_wp; intros Hlookup Hpat.
+    unfold pattern; intros Hlookup Hpat.
     simpl_extend; rewrite Hlookup. cbn; rewrite bind_ret.
     unfold locations.eqb; destruct c'; cbn.
     by rewrite Z.eqb_refl.
@@ -280,11 +289,11 @@ Section pattern_wp_rules.
   Lemma pat_PXData_neq η π p l1 l2 v φ :
     lookup_path η π = ret (VLoc l1) ->
     (address l1 <> address l2) ->
-    pattern_wp η (PXData π p) (VXData l2 v) φ True.
+    pattern η (PXData π p) (VXData l2 v) φ True.
       (* This form is useful when the truth of the equality [c = c']
         is not statically known. *)
   Proof.
-    unfold pattern_wp; intros Hlookup Heq; simpl_extend.
+    unfold pattern; intros Hlookup Heq; simpl_extend.
     rewrite Hlookup. cbn; rewrite bind_ret.
     unfold locations.eqb; simpl.
     destruct l1, l2; simpl in *.
@@ -296,11 +305,11 @@ Section pattern_wp_rules.
   Lemma pat_PXData_neq' η π p l1 l2 v :
     lookup_path η π = ret (VLoc l1) ->
     (address l1 <> address l2) ->
-    pattern_wp η (PXData π p) (VXData l2 v) (λ _, False) True.
+    pattern η (PXData π p) (VXData l2 v) (λ _, False) True.
       (* This form is useful when the truth of the equality [c = c']
         is not statically known. *)
   Proof.
-    unfold pattern_wp; intros Hlookup Heq; simpl_extend.
+    unfold pattern; intros Hlookup Heq; simpl_extend.
     rewrite Hlookup. cbn; rewrite bind_ret.
     unfold locations.eqb; simpl.
     destruct l1, l2; simpl in *.
@@ -311,22 +320,22 @@ Section pattern_wp_rules.
 
   (* -------------------------------------------------------------------------- *)
 
-  (* Syntax-directed reasoning rules for the auxiliary judgement [patterns_wp]. *)
+  (* Syntax-directed reasoning rules for the auxiliary judgement [patterns]. *)
 
   Lemma pats_PNil η φ :
     φ η →
-    patterns_wp η [] [] φ False.
+    patterns η [] [] φ False.
   Proof.
-    unfold patterns_wp.
+    unfold patterns.
     simpl_extends.
     eauto using pure_wp_ret.
   Qed.
 
   Lemma pats_PCons_unary η p ps v vs φ ψ1 ψ2 :
-    pattern_wp η p v (λ η, patterns_wp η ps vs φ ψ2) ψ1 →
-    patterns_wp η (p :: ps) (v :: vs) φ (ψ1 \/ ψ2).
+    pattern η p v (λ η, patterns η ps vs φ ψ2) ψ1 →
+    patterns η (p :: ps) (v :: vs) φ (ψ1 \/ ψ2).
   Proof.
-    unfold patterns_wp, patterns_wp. intros Hp; simpl_extends.
+    unfold patterns, patterns. intros Hp; simpl_extends.
     eapply pure_wp_bind_conseq.
     { eapply pure_wp_mono.
       - eassumption.
@@ -337,22 +346,22 @@ Section pattern_wp_rules.
   Qed.
 
   Lemma pats_PCons_unary_false η p ps v vs φ :
-    pattern_wp η p v (λ η, patterns_wp η ps vs φ False) False ->
-    patterns_wp η (p :: ps) (v :: vs) φ False.
+    pattern η p v (λ η, patterns η ps vs φ False) False ->
+    patterns η (p :: ps) (v :: vs) φ False.
   Proof.
     intros.
     assert (False \/ False -> False) as HFalse by tauto.
-    eapply patterns_wp_exn_mono; [ clear HFalse | exact HFalse ].
+    eapply patterns_exn_mono; [ clear HFalse | exact HFalse ].
     by apply pats_PCons_unary.
   Qed.
 
   Lemma pats_PCons η p ps v vs φ' φ ψ1 ψ2 :
-    pattern_wp η p v φ' ψ1 →
-    (∀ η, φ' η → patterns_wp η ps vs φ ψ2) →
-    patterns_wp η (p :: ps) (v :: vs) φ (ψ1 ∨ ψ2).
+    pattern η p v φ' ψ1 →
+    (∀ η, φ' η → patterns η ps vs φ ψ2) →
+    patterns η (p :: ps) (v :: vs) φ (ψ1 ∨ ψ2).
   Proof.
     intros. eapply pats_PCons_unary.
-    eapply pattern_wp_mono; eauto.
+    eapply pattern_mono; eauto.
   Qed.
 
   (* -------------------------------------------------------------------------- *)
@@ -367,11 +376,11 @@ Section pattern_wp_rules.
 
   Lemma pat_PConst η c c' φ :
     (c = c' -> φ η) ->
-    pattern_wp η (PConstant c) (VConstant c') φ (c <> c').
+    pattern η (PConstant c) (VConstant c') φ (c <> c').
   Proof.
     intros Hφ.
-    eapply pattern_wp_mono.
-    { eapply pat_PData.
+    eapply pattern_mono.
+    { eapply pat_PData_or.
       intros Hc; specialize (Hφ Hc).
       pats. }
     { tauto. }
@@ -380,19 +389,19 @@ Section pattern_wp_rules.
 
   Lemma pat_PConst_eq η c φ :
     φ η ->
-    pattern_wp η (PConstant c) (VConstant c) φ False.
+    pattern η (PConstant c) (VConstant c) φ False.
   Proof.
     intros Hφ.
-    eapply pattern_wp_exn_mono; [ eapply pat_PConst; eauto | tauto ].
+    eapply pattern_exn_mono; [ eapply pat_PConst; eauto | tauto ].
   Qed.
 
   Lemma pat_PConst_neq η c c' e ψ :
     c <> c' ->
     ψ ->
-    pattern_wp η (PConstant c) (VData c' e) (λ _, False) ψ.
+    pattern η (PConstant c) (VData c' e) (λ _, False) ψ.
   Proof.
     intros Hneq Hψ.
-    unfold pattern_wp. simpl_extend.
+    unfold pattern. simpl_extend.
     apply String.eqb_neq in Hneq as ->.
     by apply pure_wp_throw.
   Qed.
@@ -400,17 +409,17 @@ Section pattern_wp_rules.
   Lemma pat_false η v (P : Prop) φ :
     v = #P →
     (¬P → φ η) →
-    pattern_wp η (PConstant "false") v φ P.
+    pattern η (PConstant "false") v φ P.
   Proof.
     intros -> ?; simpl.
     destruct (truth P) eqn:?.
 
-    { eapply pattern_wp_env_mono.
+    { eapply pattern_env_mono.
       eapply pat_PConst_neq;
         [ by simpl | by apply truth_true_elim].
       done. }
 
-    { eapply pattern_wp_exn_mono.
+    { eapply pattern_exn_mono.
       eapply pat_PConst_eq;
         auto using truth_false_elim.
       tauto. }
@@ -419,17 +428,17 @@ Section pattern_wp_rules.
   Lemma pat_true η v (P : Prop) φ :
     v = #P →
     (P → φ η) →
-    pattern_wp η (PConstant "true") v φ (¬P).
+    pattern η (PConstant "true") v φ (¬P).
   Proof.
     intros -> Hφ; simpl.
     destruct (truth P) eqn:?.
 
-    { eapply pattern_wp_exn_mono.
+    { eapply pattern_exn_mono.
       eapply pat_PConst_eq;
         apply Hφ; by apply truth_true_elim.
       tauto. }
 
-    { eapply pattern_wp_env_mono.
+    { eapply pattern_env_mono.
       eapply pat_PConst_neq;
         [ by simpl | by apply truth_false_elim].
       intros; tauto. }
@@ -440,10 +449,10 @@ Section pattern_wp_rules.
     int.representable j →
     v = #j →
     (i = j → φ η) →
-    pattern_wp η (PInt i) v φ (i <> j).
+    pattern η (PInt i) v φ (i <> j).
   Proof.
     intros Hi Hj -> Hφ.
-    unfold pattern_wp; simpl_extend.
+    unfold pattern; simpl_extend.
     rewrite int.eq_repr_repr; auto.
     destruct (_ =? _) eqn:E.
     - apply pure_wp_ret. apply Hφ. by apply Z.eqb_eq.
@@ -453,53 +462,53 @@ Section pattern_wp_rules.
   (* -------------------------------------------------------------------------- *)
 
   Lemma cpat_CVal η p v φ ψ :
-    pattern_wp η p v φ ψ ->
-    cpattern_wp η (CVal p) (O2Ret v) φ ψ.
+    pattern η p v φ ψ ->
+    cpattern η (CVal p) (O2Ret v) φ ψ.
   Proof.
     tauto.
   Qed.
 
   Lemma cpat_CExc η p v φ ψ :
-    pattern_wp η p v φ ψ ->
-    cpattern_wp η (CExc p) (O2Throw v) φ ψ.
+    pattern η p v φ ψ ->
+    cpattern η (CExc p) (O2Throw v) φ ψ.
   Proof.
     tauto.
   Qed.
 
   Lemma cpat_COr η cp1 cp2 o φ ψ1 ψ2 :
-    cpattern_wp η cp1 o φ ψ1 ->
-    cpattern_wp η cp2 o φ ψ2 ->
-    cpattern_wp η (COr cp1 cp2) o φ (ψ1 /\ ψ2).
+    cpattern η cp1 o φ ψ1 ->
+    cpattern η cp2 o φ ψ2 ->
+    cpattern η (COr cp1 cp2) o φ (ψ1 /\ ψ2).
   Proof.
-    unfold cpattern_wp. intros.
+    unfold cpattern. intros.
     eapply pure_wp_orelse; [ eassumption | ].
     eauto using pure_wp_mono.
   Qed.
 
   Lemma cpat_CEff η peff pk v k φ ψ1 ψ2 :
-    pattern_wp η peff v (λ δ, pattern_wp δ pk (VCont k) φ ψ2) ψ1 ->
-    cpattern_wp η (CEff peff pk) (O3Perform v k) φ (ψ1 \/ ψ2).
+    pattern η peff v (λ δ, pattern δ pk (VCont k) φ ψ2) ψ1 ->
+    cpattern η (CEff peff pk) (O3Perform v k) φ (ψ1 \/ ψ2).
   Proof.
-    unfold cpattern_wp, pattern_wp; intros. simpl.
+    unfold cpattern, pattern; intros. simpl.
     eapply pure_wp_bind_conseq; [ eapply pure_wp_mono; eauto | ].
     simpl; intros δ ?.
     eauto using pure_wp_mono.
   Qed.
 
-  Fixpoint valid_cpattern_wp_match {A E} cp (o : outcome3 A E) :=
+  Fixpoint valid_cpattern_match {A E} cp (o : outcome3 A E) :=
     match cp, o with
     | CVal _, O3Ret _
     | CExc _, O3Throw _
     | CEff _ _, O3Perform _ _ =>
         true
     | COr cp1 cp2, _ =>
-        valid_cpattern_wp_match cp1 o || valid_cpattern_wp_match cp2 o
+        valid_cpattern_match cp1 o || valid_cpattern_match cp2 o
     | _, _ =>
         false
     end.
 
   Lemma invert_valid_match cp o :
-    valid_cpattern_wp_match cp o = false ->
+    valid_cpattern_match cp o = false ->
     ∀ η, cextend η cp o = throw ().
   Proof.
     intros Hvalid η.
@@ -512,12 +521,12 @@ Section pattern_wp_rules.
   Qed.
 
   Lemma cpat_mismatch η cp o φ (ψ : Prop) :
-    valid_cpattern_wp_match cp o = false ->
+    valid_cpattern_match cp o = false ->
     ψ ->
-    cpattern_wp η cp o φ ψ.
+    cpattern η cp o φ ψ.
   Proof.
     intros.
-    unfold cpattern_wp.
+    unfold cpattern.
     rewrite invert_valid_match by assumption.
     by apply pure_wp_throw.
   Qed.
@@ -533,12 +542,12 @@ Section pattern_wp_rules.
     v = #xs →
     (xs = [] -> φ η) →
     (* Enter the branch with knowledge that [xs] is empty *)
-    pattern_wp η pNil v φ (xs ≠ []).
+    pattern η pNil v φ (xs ≠ []).
     (* If the match is unsuccessful, move to the next branch
       with the knowledge that [xs] is not empty *)
   Proof.
     intros; subst.
-    destruct xs; eapply pattern_wp_exn_mono.
+    destruct xs; eapply pattern_exn_mono.
     { eapply pat_PConst; eauto. }
     { tauto. }
     { eapply pat_PData_neq; done. }
@@ -555,14 +564,14 @@ Section pattern_wp_rules.
     v = #xs ->
     (∀ (x : A) (xs' : list A),
         xs = x :: xs' →
-        pattern_wp η p1 #x (φ1 x) (ψ1 x)) ->
+        pattern η p1 #x (φ1 x) (ψ1 x)) ->
         (* If [#x] matches [p1], we gain the knowledge [φ1 x η0].
           Otherwise, we gain the knowledge [ψ1 x] *)
     (∀ (x : A) (xs' : list A),
         xs = x :: xs' →
-        (forall η', φ1 x η' -> pattern_wp η' p2 #xs' φ (ψ2 xs'))) ->
+        (forall η', φ1 x η' -> pattern η' p2 #xs' φ (ψ2 xs'))) ->
         (* If [#xs'] does not match [p2], then we gain the knowledge [ψ2 xs'] *)
-    pattern_wp η (pCons p1 p2) v φ (xs = [] \/ (exists x xs', xs = x :: xs' /\ (ψ1 x \/ ψ2 xs'))).
+    pattern η (pCons p1 p2) v φ (xs = [] \/ (exists x xs', xs = x :: xs' /\ (ψ1 x \/ ψ2 xs'))).
     (* There are three ways the match can be unsuccessful:
       - the list is empty
       - the list is non-empty, but its head did not match [p1]
@@ -570,10 +579,10 @@ Section pattern_wp_rules.
   Proof.
     intros; subst.
     destruct xs.
-    { eapply pattern_wp_exn_mono.
+    { eapply pattern_exn_mono.
       { by apply pat_PData_neq. }
       tauto. }
-    { eapply pattern_wp_exn_mono.
+    { eapply pattern_exn_mono.
       { eapply pat_PData_eq; pats.  }
       right; do 2 eexists; split; [ reflexivity | tauto ]. }
   Qed.
@@ -584,34 +593,28 @@ Section pattern_wp_rules.
     v = #xs ->
     (∀ (x : A) (xs' : list A),
         xs = x :: xs' →
-        pattern_wp η p1 #x
+        pattern η p1 #x
           (λ η',
-            pattern_wp η' p2 #xs' φ (ψ2 xs'))
+            pattern η' p2 #xs' φ (ψ2 xs'))
           (ψ1 x)) ->
-    pattern_wp η (pCons p1 p2) v φ
+    pattern η (pCons p1 p2) v φ
       (xs = [] \/ (exists x xs', xs = x :: xs' /\ (ψ1 x \/ ψ2 xs'))).
   Proof.
     intros; subst.
-    destruct xs; eapply pattern_wp_exn_mono.
+    destruct xs; eapply pattern_exn_mono.
     { by apply pat_PData_neq. }
     { tauto. }
     { eapply pat_PData_eq; pats. }
     { clear; right; do 2 eexists; split; [ reflexivity | tauto ]. }
   Qed.
 
-  Local Ltac pat_pNil :=
-    eapply pat_pNil; first solve [ encode ].
-
-  Local Ltac pat_pCons :=
-    eapply pat_pCons; first solve [ encode ].
-
   (* The previous lemmas start to give us a general scheme for reasoning about
-    pattern_wp matching on ADTs.
+    pattern matching on ADTs.
 
     More experimenting is required.
     As of now (29/02/24), see [examples/splay.v] for more examples. *)
 
-  (* Pattern_Wp proofmode tactics *)
+  (* Pattern proofmode tactics *)
 
 
   Definition is_not_O3Throw {A X} (o : outcome3 A X) :=
@@ -633,11 +636,11 @@ Section pattern_wp_rules.
     end.
 
   Lemma cpat_CExc_abst η p o φ ψ :
-    (forall e, o = O3Throw e -> pattern_wp η p e φ ψ) ->
-    cpattern_wp η (CExc p) o φ (is_not_O3Throw o ∨ ψ).
+    (forall e, o = O3Throw e -> pattern η p e φ ψ) ->
+    cpattern η (CExc p) o φ (is_not_O3Throw o ∨ ψ).
   Proof.
     intros Hpat.
-    unfold cpattern_wp.
+    unfold cpattern.
     destruct o; simpl.
     - apply pure_wp_throw. by left.
     - eapply pure_wp_mono; [ apply Hpat | auto | auto ].
@@ -646,11 +649,11 @@ Section pattern_wp_rules.
   Qed.
 
   Lemma cpat_CVal_abst η p o φ ψ :
-    (forall v, o = O3Ret v -> pattern_wp η p v φ ψ) ->
-    cpattern_wp η (CVal p) o φ (is_not_O3Ret o ∨ ψ).
+    (forall v, o = O3Ret v -> pattern η p v φ ψ) ->
+    cpattern η (CVal p) o φ (is_not_O3Ret o ∨ ψ).
   Proof.
     intros Hpat.
-    unfold cpattern_wp.
+    unfold cpattern.
     destruct o; simpl.
     - eapply pure_wp_mono; [ apply Hpat | auto | auto ].
       reflexivity.
@@ -661,11 +664,11 @@ Section pattern_wp_rules.
   Lemma cpat_CEff_abst η peff pk o φ ψ1 ψ2 :
     (forall eff k,
         o = O3Perform eff k ->
-        pattern_wp η peff eff (λ δ, pattern_wp δ pk (VCont k) φ ψ2) ψ1) ->
-    cpattern_wp η (CEff peff pk) o φ (is_not_O3Perform o ∨ ψ1 ∨ ψ2).
+        pattern η peff eff (λ δ, pattern δ pk (VCont k) φ ψ2) ψ1) ->
+    cpattern η (CEff peff pk) o φ (is_not_O3Perform o ∨ ψ1 ∨ ψ2).
   Proof.
     intros Hpat.
-    unfold cpattern_wp.
+    unfold cpattern.
     destruct o; simpl.
     - apply pure_wp_throw. by left.
     - apply pure_wp_throw. by left.
@@ -676,200 +679,10 @@ Section pattern_wp_rules.
   Qed.
 
   Lemma cpat_CEff_impossible η peff pk (o : outcome2 val exn) φ :
-    cpattern_wp η (CEff peff pk) o φ True.
+    cpattern η (CEff peff pk) o φ True.
   Proof.
-    unfold cpattern_wp.
+    unfold cpattern.
     destruct o; simpl; by apply pure_wp_throw.
   Qed.
 
-End pattern_wp_rules.
-
-Create HintDb pat.
-
-#[global] Hint Immediate pat_PAny pat_PVar pat_PVar2 pat_PAlias pat_POr pat_PUnit pat_PTuple pat_PTuple_val pat_PPair pat_PData pat_PData_eq pat_PData_neq pat_PXData_eq pat_PXData_neq pat_PXData_neq' pats_PNil pats_PCons_unary pats_PCons_unary_false pats_PCons pat_PConst pat_PConst_eq pat_PConst_neq pat_false pat_true pat_PInt cpat_CVal cpat_CExc cpat_COr cpat_CEff pat_pNil pat_pCons pat_pCons_cut : pat.
-
-Section pattern_constructors.
-
-Implicit Type φ : env -> Prop.
-Implicit Type ψ : Prop.
-
-Inductive pattern : env -> pat -> val -> (env -> Prop) -> Prop -> Prop :=
-  | pattern_PAny φ η v :
-      φ η →
-      pattern η PAny v φ False
-  | pattern_PVar x φ η v :
-      φ ((x, v) :: η) →
-      pattern η (PVar x) v φ False
-  | pattern_PVar2 x η v :
-      pattern η (PVar x) v (λ η', η' = (x, v) :: η) False
-  | pattern_PAlias p x φ ψ η v :
-      pattern η p v (λ η', φ ((x, v) :: η')) ψ →
-      pattern η (PAlias p x) v φ ψ
-  | pattern_POr p1 p2 φ ψ1 ψ2 η v :
-      pattern η p1 v φ ψ1 →
-      pattern η p2 v φ ψ2 →
-      pattern η (POr p1 p2) v φ (ψ1 ∧ ψ2)
-  | pattern_PUnit η v φ :
-      φ η →
-      v = #() →
-      pattern η PUnit v φ False
-  | pattern_PTuple {A} `{Encode A} ps vs φ ψ η (a : A) :
-      #a = VTuple vs →
-      patterns_wp η ps vs φ ψ →
-      pattern η (PTuple ps) #a φ ψ
-  | pattern_PTuple_val ps vs φ ψ η :
-      patterns_wp η ps vs φ ψ →
-      pattern η (PTuple ps) (VTuple vs) φ ψ
-  | pattern_PPair
-      `{Encode A, Encode B}
-      p1 p2 ψ1 ψ2 φ φ' η v1 v2
-      (x1 : A) (x2 : B) :
-      v1 = #x1 →
-      v2 = #x2 →
-      (forall η', φ' η' -> pattern η' p2 #x2 φ ψ2) ->
-      pattern η p1 #x1 φ' ψ1 →
-      pattern η (PPair p1 p2) (VPair v1 v2) φ (ψ1 ∨ ψ2)
-  | pattern_PData_nil c φ η :
-    φ η ->
-    pattern η (PData c nil) (VData c nil) φ False
-  | pattern_PData_eq c p v φ ψ η :
-      patterns_wp η p v φ ψ →
-      pattern η (PData c p) (VData c v) φ ψ
-  | pattern_PData_neq c p c' v φ η ψ:
-      c ≠ c' →
-      ψ ->
-      pattern η (PData c p) (VData c' v) φ ψ
-  | pattern_PData c p c' v φ ψ η :
-      (c = c' → patterns_wp η p v φ ψ) →
-      pattern η (PData c p) (VData c' v) φ (ψ ∨ c ≠ c')
-  | pattern_PXData_eq π p (c c' : loc) v φ ψ η :
-      lookup_path η π = ret (VLoc c') →
-      patterns_wp η p v φ ψ →
-      pattern η (PXData π p) (VXData c' v) φ ψ
-  | pattern_PXData_neq π p l1 l2 v φ η ψ:
-      lookup_path η π = ret (VLoc l1) →
-      (address l1 ≠ address l2) →
-      ψ ->
-      pattern η (PXData π p) (VXData l2 v) φ ψ
-  | pattern_PXData_neq' π p l1 l2 v η ψ:
-      lookup_path η π = ret (VLoc l1) →
-      (address l1 ≠ address l2) →
-      ψ ->
-      pattern η (PXData π p) (VXData l2 v) (λ _, False) ψ
-  | pattern_Base φ p η v ψ:
-      pattern_wp η p v φ ψ ->
-      pattern η p v φ ψ.
-
-Lemma pattern_equals_pat p η v φ ψ:
-  pattern η p v φ ψ <->
-  pattern_wp η p v φ ψ.
-Proof.
-  intros; split; [ | by constructor ].
-  intros; induction H; eauto with pat.
-  eapply pat_PPair; eauto.
-  eapply pattern_wp_mono; eauto.
-  all: eapply pattern_wp_mono; eauto with pat; try firstorder.
-Qed.
-
-Inductive cpattern : env -> cpat -> outcome.outcome3 val loc val val -> (env -> Prop) -> Prop -> Prop :=
-  | cpattern_CVal p v φ ψ η :
-      pattern η p v φ ψ →
-      cpattern η (CVal p) (O2Ret v) φ ψ
-  | cpattern_CExc p v φ ψ η :
-      pattern η p v φ ψ →
-      cpattern η (CExc p) (O2Throw v) φ ψ
-  | cpattern_COr cp1 cp2 o φ ψ1 ψ2 η :
-      cpattern η cp1 o φ ψ1 →
-      cpattern η cp2 o φ ψ2 →
-      cpattern η (COr cp1 cp2) o φ (ψ1 ∧ ψ2)
-  | cpattern_CEff peff pk v k φ ψ1 ψ2 η :
-      pattern η peff v (λ δ, pattern δ pk (VCont k) φ ψ2) ψ1 →
-      cpattern η (CEff peff pk) (O3Perform v k) φ (ψ1 ∨ ψ2)
-  | cpattern_Base φ p η v ψ:
-      cpattern_wp η p v φ ψ ->
-      cpattern η p v φ ψ.
-
-Lemma cpattern_equals_cpat p η v φ ψ:
-  cpattern η p v φ ψ <->
-  cpattern_wp η p v φ ψ.
-Proof.
-  intros; split; [ | by constructor ].
-  intros; induction H; try apply pattern_equals_pat; eauto with pat.
-  apply cpat_CEff; eapply pattern_wp_mono; eauto.
-  by apply pattern_equals_pat.
-  intros; by apply pattern_equals_pat.
-Qed.
-
-Inductive patterns : env -> list pat -> list val -> (env -> Prop) -> Prop -> Prop :=
-  | patterns_PNil φ ψ η :
-      φ η →
-      (ψ -> False) ->
-      patterns η [] [] φ ψ
-  | patterns_PCons_unary_or p ps v vs φ φ' ψ1 ψ2 η :
-      (forall η', φ' η' -> patterns η' ps vs φ ψ2) ->
-      pattern η p v φ' ψ1 →
-      patterns η (p :: ps) (v :: vs) φ (ψ1 ∨ ψ2)
-  | patterns_PCons_unary_false p ps v vs φ φ' η :
-      (forall η', φ' η' -> patterns η' ps vs φ False) ->
-      pattern η p v φ' False →
-      patterns η (p :: ps) (v :: vs) φ False
-  | patterns_PCons p ps v vs φ' φ ψ1 ψ2 η :
-      pattern η p v φ' ψ1 →
-      (∀ η', φ' η' → patterns η' ps vs φ ψ2) →
-      patterns η (p :: ps) (v :: vs) φ (ψ1 ∨ ψ2)
-  | patterns_Base φ p η v ψ:
-      patterns_wp η p v φ ψ ->
-      patterns η p v φ ψ.
-
-Lemma patterns_equals_pats p η v φ ψ:
-  patterns η p v φ ψ <->
-  patterns_wp η p v φ ψ.
-Proof.
-  intros; split; [ | by constructor ].
-  intros; induction H; eauto with pat.
-  - eapply patterns_wp_mono. apply pats_PNil. all: eauto. intros; done.
-  - eapply pats_PCons; first by apply pattern_equals_pat; intros; eauto.
-    intros; auto.
-  - eapply pats_PCons_unary_false.
-    eapply pattern_wp_mono; eauto.
-    by apply pattern_equals_pat.
-  - eapply pats_PCons.
-    by apply pattern_equals_pat.
-    intros; auto.
-Qed.
-
-End pattern_constructors.
-
-Global Hint Resolve pattern_PAny pattern_PVar pattern_PVar2 pattern_PAlias pattern_POr pattern_PUnit pattern_PTuple pattern_PTuple_val pattern_PPair pattern_PData pattern_PData_eq pattern_PData_neq : pat.
-Global Hint Resolve cpattern_CVal cpattern_CExc cpattern_COr cpattern_CEff : pat.
-Global Hint Resolve patterns_PNil patterns_PCons_unary_or patterns_PCons_unary_false patterns_PCons : pat.
-
-#[global]
-  Hint Extern 2 (patterns_wp _ _ _ _ _) => apply patterns_equals_pats; eauto with pat: pat.
-#[global]
-  Hint Extern 2 (pattern _ _ _ _ _) => econstructor; eauto : pat.
-
-Ltac eauto_pattern := by eauto with pat.
-
-Ltac normalize_pattern :=
-  try
-  match goal with
-  | |- pattern_wp _ _ _ _ _ => apply pattern_equals_pat
-  | |- patterns_wp _ _ _ _ _ => apply patterns_equals_pats
-  | |- cpattern_wp _ _ _ _ _ => apply cpattern_equals_cpat
-  end.
-
-Ltac solve_pattern :=
-  repeat
-    match goal with
-    | |- cpattern _ _ _ _ _ => econstructor; eauto
-    | |- pattern _ _ _ _ _ => econstructor; eauto
-    | |- patterns _ (_ :: _) (_ :: _) _ _ =>
-        let η := fresh "η" in
-        eapply patterns_PCons; [ eauto_pattern | .. ];
-          intros η ->
-    | |- patterns _ [] [] _ _ =>
-        try (apply (patterns_PNil _ False); last done)
-    | |- patterns_wp _ _ _ _ _ => apply patterns_equals_pats
-    end;
-  normalize_pattern.
+End pattern_rules.
