coq-osiris/theories/program_logic/pure/eval_tactics.v
@@ -1,0 +1,4 @@
+From osiris Require Import base.
+From osiris.lang Require Import lang.
+From osiris.semantics Require Import semantics.
+From osiris.program_logic.pure Require Import eval_rules pattern_rules.
