coq-osiris/theories/program_logic/pure/pure.v
@@ -4,8 +4,8 @@ From osiris.program_logic.pure Require Export
      notation
      pure_rules
      total_rules
+     simp_tactics
      eval_rules
      pattern_rules
      struct_rules
-     simp_tactics
      .
